@prefix : <http://purl.org/spar/bido/> .
@prefix dc: <http://purl.org/dc/elements/1.1/> .
@prefix fabio: <http://purl.org/spar/fabio/> .
@prefix owl: <http://www.w3.org/2002/07/owl#> .
@prefix rdf: <http://www.w3.org/1999/02/22-rdf-syntax-ns#> .
@prefix rdfs: <http://www.w3.org/2000/01/rdf-schema#> .
@prefix skos: <http://www.w3.org/2004/02/skos/core#> .
@prefix swc: <http://data.semanticweb.org/ns/swc/ontology#> .
@prefix xml: <http://www.w3.org/XML/1998/namespace> .
@prefix xsd: <http://www.w3.org/2001/XMLSchema#> .

<http://purl.org/NET/rdflicense/cc-by4.0> a owl:NamedIndividual .

:a-r-ts-rejps a :ReviewRatingValue,
        owl:NamedIndividual ;
    rdfs:label "Reject, Pre-Screening (Accept to Reject, Two Strikes review rating scale)"@en ;
    rdfs:isDefinedBy <http://purl.org/spar/bido-review-measures> ;
    skos:inScheme :a-r-ts .

:a-r-ts-rejts a :ReviewRatingValue,
        owl:NamedIndividual ;
    rdfs:label "Reject, Two Strikes (Accept to Reject, Two Strikes review rating scale)"@en ;
    rdfs:isDefinedBy <http://purl.org/spar/bido-review-measures> ;
    skos:inScheme :a-r-ts .

:average-of-reviews-per-paper a [ a owl:Restriction ;
            owl:allValuesFrom [ a owl:Restriction ;
                    owl:allValuesFrom [ a owl:Restriction ;
                            owl:allValuesFrom [ a owl:Class ;
                                    owl:unionOf ( swc:AcademicEvent fabio:Expression ) ] ;
                            owl:onProperty [ owl:inverseOf :holdsBibliometricDataInTime ] ] ;
                    owl:onProperty [ owl:inverseOf :withBibliometricData ] ] ;
            owl:onProperty [ owl:inverseOf :hasMeasure ] ],
        :BibliometricMeasure,
        owl:NamedIndividual ;
    rdfs:label "average number of reviews per paper" ;
    rdfs:comment "It indicates how many reviewers has been used for each paper submitted to a venue." ;
    rdfs:isDefinedBy <http://purl.org/spar/bido-review-measures> .

:conference-management-toolkit a :ScholarlyVenueManagementSystem,
        owl:NamedIndividual ;
    rdfs:label "Conference Management Toolkit" ;
    rdfs:comment "The Conference Management Toolkit (CMT) is a free conference management service sponsored by Microsoft Research." ;
    rdfs:isDefinedBy <http://purl.org/spar/bido-review-measures> .

:core-a-star a :ConferenceRankingCategory,
        owl:NamedIndividual ;
    rdfs:label "A*" ;
    :isDefinedIn :core-conference-ranking ;
    :isHigherThan :core-a ;
    rdfs:comment "The CORE category for a flagship conference, a leading venue in a discipline area." ;
    rdfs:isDefinedBy <http://purl.org/spar/bido-review-measures> .

:demo-paper-accepted a [ a owl:Restriction ;
            owl:allValuesFrom [ a owl:Restriction ;
                    owl:allValuesFrom [ a owl:Restriction ;
                            owl:allValuesFrom [ a owl:Class ;
                                    owl:unionOf ( swc:AcademicEvent fabio:Expression ) ] ;
                            owl:onProperty [ owl:inverseOf :holdsBibliometricDataInTime ] ] ;
                    owl:onProperty [ owl:inverseOf :withBibliometricData ] ] ;
            owl:onProperty [ owl:inverseOf :hasMeasure ] ],
        :BibliometricMeasure,
        owl:NamedIndividual ;
    rdfs:label "number of demo paper accepted" ;
    rdfs:comment "It indicates how many demo papers has been accepted for publication/presentation in the venue." ;
    rdfs:isDefinedBy <http://purl.org/spar/bido-review-measures> .

:dis-0-10-1 a :ReviewRatingValue,
        owl:NamedIndividual ;
    rdfs:label "1 out of 10 (Discrete 0 to 10 review rating scale)"@en ;
    :hasRatingValue "1"^^xsd:int ;
    rdfs:isDefinedBy <http://purl.org/spar/bido-review-measures> ;
    skos:inScheme :dis-0-10 .

:dis-0-10-2 a :ReviewRatingValue,
        owl:NamedIndividual ;
    rdfs:label "2 out of 10 (Discrete 0 to 10 review rating scale)"@en ;
    :hasRatingValue "2"^^xsd:int ;
    rdfs:isDefinedBy <http://purl.org/spar/bido-review-measures> ;
    skos:inScheme :dis-0-10 .

:dis-0-10-3 a :ReviewRatingValue,
        owl:NamedIndividual ;
    rdfs:label "3 out of 10 (Discrete 0 to 10 review rating scale)"@en ;
    :hasRatingValue "3"^^xsd:int ;
    rdfs:isDefinedBy <http://purl.org/spar/bido-review-measures> ;
    skos:inScheme :dis-0-10 .

:dis-0-10-4 a :ReviewRatingValue,
        owl:NamedIndividual ;
    rdfs:label "4 out of 10 (Discrete 0 to 10 review rating scale)"@en ;
    :hasRatingValue "4"^^xsd:int ;
    rdfs:isDefinedBy <http://purl.org/spar/bido-review-measures> ;
    skos:inScheme :dis-0-10 .

:dis-0-10-6 a :ReviewRatingValue,
        owl:NamedIndividual ;
    rdfs:label "6 out of 10 (Discrete 0 to 10 review rating scale)"@en ;
    :hasRatingValue "6"^^xsd:int ;
    rdfs:isDefinedBy <http://purl.org/spar/bido-review-measures> ;
    skos:inScheme :dis-0-10 .

:dis-0-10-7 a :ReviewRatingValue,
        owl:NamedIndividual ;
    rdfs:label "7 out of 10 (Discrete 0 to 10 review rating scale)"@en ;
    :hasRatingValue "7"^^xsd:int ;
    rdfs:isDefinedBy <http://purl.org/spar/bido-review-measures> ;
    skos:inScheme :dis-0-10 .

:dis-0-10-8 a :ReviewRatingValue,
        owl:NamedIndividual ;
    rdfs:label "8 out of 10 (Discrete 0 to 10 review rating scale)"@en ;
    :hasRatingValue "8"^^xsd:int ;
    rdfs:isDefinedBy <http://purl.org/spar/bido-review-measures> ;
    skos:inScheme :dis-0-10 .

:dis-0-10-9 a :ReviewRatingValue,
        owl:NamedIndividual ;
    rdfs:label "9 out of 10 (Discrete 0 to 10 review rating scale)"@en ;
    :hasRatingValue "9"^^xsd:int ;
    rdfs:isDefinedBy <http://purl.org/spar/bido-review-measures> ;
    skos:inScheme :dis-0-10 .

:double-blind-peer-review a :PeerReviewType,
        owl:NamedIndividual ;
    rdfs:label "double blind peer review" ;
    rdfs:comment "It identifies all the review processes where the identity of the authors is concealed from the reviewers, and vice versa." ;
    rdfs:isDefinedBy <http://purl.org/spar/bido-review-measures> .

:easychair a :ScholarlyVenueManagementSystem,
        owl:NamedIndividual ;
    rdfs:label "EasyChair" ;
    rdfs:comment "EasyChair is a conference management system that is flexible, easy to use, and has many features to make it suitable for various conference models. It is currently probably the most commonly used conference management system." ;
    rdfs:isDefinedBy <http://purl.org/spar/bido-review-measures> .

:external-reviewers-involved a [ a owl:Restriction ;
            owl:allValuesFrom [ a owl:Restriction ;
                    owl:allValuesFrom [ a owl:Restriction ;
                            owl:allValuesFrom [ a owl:Class ;
                                    owl:unionOf ( swc:AcademicEvent fabio:Expression ) ] ;
                            owl:onProperty [ owl:inverseOf :holdsBibliometricDataInTime ] ] ;
                    owl:onProperty [ owl:inverseOf :withBibliometricData ] ] ;
            owl:onProperty [ owl:inverseOf :hasMeasure ] ],
        :BibliometricMeasure,
        owl:NamedIndividual ;
    rdfs:label "number of external reviewers involved" ;
    rdfs:comment "It indicates how many external reviewers have been involved in the reviewing phase." ;
    rdfs:isDefinedBy <http://purl.org/spar/bido-review-measures> .

:full-papers-accepted a [ a owl:Restriction ;
            owl:allValuesFrom [ a owl:Restriction ;
                    owl:allValuesFrom [ a owl:Restriction ;
                            owl:allValuesFrom [ a owl:Class ;
                                    owl:unionOf ( swc:AcademicEvent fabio:Expression ) ] ;
                            owl:onProperty [ owl:inverseOf :holdsBibliometricDataInTime ] ] ;
                    owl:onProperty [ owl:inverseOf :withBibliometricData ] ] ;
            owl:onProperty [ owl:inverseOf :hasMeasure ] ],
        :BibliometricMeasure,
        owl:NamedIndividual ;
    rdfs:label "number of full paper accepted" ;
    rdfs:comment "It indicates how many full papers has been accepted for publication/presentation in the venue." ;
    rdfs:isDefinedBy <http://purl.org/spar/bido-review-measures> .

:hasConfidenceValue a owl:DatatypeProperty ;
    rdfs:label "has confidence value"@en ;
    rdfs:comment "The confidence value of expertise in the review topic given by the reviwer."@en ;
    rdfs:domain :ReviewerConfidenceValue ;
    rdfs:isDefinedBy <http://purl.org/spar/bido-review-measures> ;
    rdfs:range rdfs:Literal .

:hasRatingValue a owl:DatatypeProperty ;
    rdfs:label "has rating value"@en ;
    rdfs:comment "The value of the rating given to a review."@en ;
    rdfs:domain :ReviewRatingValue ;
    rdfs:isDefinedBy <http://purl.org/spar/bido-review-measures> ;
    rdfs:range rdfs:Literal .

:isDefinedIn a owl:ObjectProperty ;
    rdfs:label "is defined in ranking" ;
    rdfs:comment "It links a ranking category with the ranking that defines it." ;
    rdfs:domain :CategorialBibliometricData ;
    rdfs:isDefinedBy <http://purl.org/spar/bido-review-measures> ;
    rdfs:range skos:ConceptScheme ;
    rdfs:subPropertyOf skos:inScheme .

:isHigherThan a owl:ObjectProperty ;
    rdfs:label "is higher than" ;
    rdfs:comment "It links a ranking category with one that is less important." ;
    rdfs:domain :CategorialBibliometricData ;
    rdfs:isDefinedBy <http://purl.org/spar/bido-review-measures> ;
    rdfs:range :CategorialBibliometricData ;
    owl:inverseOf :isLowerThan .

:open-peer-review a :PeerReviewType,
        owl:NamedIndividual ;
    rdfs:label "open peer review" ;
    rdfs:comment "It identifies all the review processes where the identity of the authors and the reviewers is known." ;
    rdfs:isDefinedBy <http://purl.org/spar/bido-review-measures> .

:poster-papers-accepted a [ a owl:Restriction ;
            owl:allValuesFrom [ a owl:Restriction ;
                    owl:allValuesFrom [ a owl:Restriction ;
                            owl:allValuesFrom [ a owl:Class ;
                                    owl:unionOf ( swc:AcademicEvent fabio:Expression ) ] ;
                            owl:onProperty [ owl:inverseOf :holdsBibliometricDataInTime ] ] ;
                    owl:onProperty [ owl:inverseOf :withBibliometricData ] ] ;
            owl:onProperty [ owl:inverseOf :hasMeasure ] ],
        :BibliometricMeasure,
        owl:NamedIndividual ;
    rdfs:label "number of poster paper accepted" ;
    rdfs:comment "It indicates how many poster papers has been accepted for publication/presentation in the venue." ;
    rdfs:isDefinedBy <http://purl.org/spar/bido-review-measures> .

:short-papers-accepted a [ a owl:Restriction ;
            owl:allValuesFrom [ a owl:Restriction ;
                    owl:allValuesFrom [ a owl:Restriction ;
                            owl:allValuesFrom [ a owl:Class ;
                                    owl:unionOf ( swc:AcademicEvent fabio:Expression ) ] ;
                            owl:onProperty [ owl:inverseOf :holdsBibliometricDataInTime ] ] ;
                    owl:onProperty [ owl:inverseOf :withBibliometricData ] ] ;
            owl:onProperty [ owl:inverseOf :hasMeasure ] ],
        :BibliometricMeasure,
        owl:NamedIndividual ;
    rdfs:label "number of short paper accepted" ;
    rdfs:comment "It indicates how many short papers has been accepted for publication/presentation in the venue." ;
    rdfs:isDefinedBy <http://purl.org/spar/bido-review-measures> .

:single-blind-peer-review a :PeerReviewType,
        owl:NamedIndividual ;
    rdfs:label "single blind peer review" ;
    rdfs:comment "It identifies all the review processes where the identity of the reviewers is concealed from the authors." ;
    rdfs:isDefinedBy <http://purl.org/spar/bido-review-measures> .

:submissions-sent-for-review a [ a owl:Restriction ;
            owl:allValuesFrom [ a owl:Restriction ;
                    owl:allValuesFrom [ a owl:Restriction ;
                            owl:allValuesFrom [ a owl:Class ;
                                    owl:unionOf ( swc:AcademicEvent fabio:Expression ) ] ;
                            owl:onProperty [ owl:inverseOf :holdsBibliometricDataInTime ] ] ;
                    owl:onProperty [ owl:inverseOf :withBibliometricData ] ] ;
            owl:onProperty [ owl:inverseOf :hasMeasure ] ],
        :BibliometricMeasure,
        owl:NamedIndividual ;
    rdfs:label "number of submission sent for review" ;
    rdfs:comment "It indicates how many submitted papers has been assagned to reviewers for revision." ;
    rdfs:isDefinedBy <http://purl.org/spar/bido-review-measures> .

:to-10-continuos a :ReviewRatingScale,
        owl:NamedIndividual ;
    rdfs:label "0 to 10 continuos review rating scale"@en ;
    rdfs:isDefinedBy <http://purl.org/spar/bido-review-measures> .

:to-15-continuos a :ReviewRatingScale,
        owl:NamedIndividual ;
    rdfs:label "0 to 15 continuos review rating scale"@en ;
    rdfs:isDefinedBy <http://purl.org/spar/bido-review-measures> .

:to-5-continuos a :ReviewRatingScale,
        owl:NamedIndividual ;
    rdfs:isDefinedBy <http://purl.org/spar/bido-review-measures> ;
    skos:prefLabel "0 to 5 continuos review rating scale"@en .

skos:closeMatch a owl:ObjectProperty ;
    rdfs:isDefinedBy <http://www.w3.org/2004/02/skos/core> .

skos:prefLabel a owl:AnnotationProperty .

:ConferenceRanking a owl:Class ;
    rdfs:label "conference ranking" ;
    rdfs:comment "This class describes conference rankings as composed by categories identifying different rankings." ;
    rdfs:isDefinedBy <http://purl.org/spar/bido-review-measures> ;
    rdfs:subClassOf skos:ConceptScheme .

:ReviewerConfidenceScale a owl:Class ;
    rdfs:label "reviewer confidence scale"@en ;
    rdfs:comment "A scale defining the confidence of a reviewer for a given topic."@en ;
    rdfs:isDefinedBy <http://purl.org/spar/bido-review-measures> ;
    rdfs:subClassOf skos:ConceptScheme .

:core-a a :ConferenceRankingCategory,
        owl:NamedIndividual ;
    rdfs:label "A" ;
    :isDefinedIn :core-conference-ranking ;
    :isHigherThan :core-b ;
    rdfs:comment "The CORE category for an excellent conference, and highly respected in a discipline area." ;
    rdfs:isDefinedBy <http://purl.org/spar/bido-review-measures> .

:core-b a :ConferenceRankingCategory,
        owl:NamedIndividual ;
    rdfs:label "B" ;
    :isDefinedIn :core-conference-ranking ;
    :isHigherThan :core-c ;
    rdfs:comment "The CORE category for a good conference, and well regarded in a discipline area." ;
    rdfs:isDefinedBy <http://purl.org/spar/bido-review-measures> .

:core-c a :ConferenceRankingCategory,
        owl:NamedIndividual ;
    rdfs:label "C" ;
    :isDefinedIn :core-conference-ranking ;
    :isHigherThan :core-unranked ;
    rdfs:comment "The CORE category for other ranked conference venues that meet minimum standards." ;
    rdfs:isDefinedBy <http://purl.org/spar/bido-review-measures> .

:core-unranked a :ConferenceRankingCategory,
        owl:NamedIndividual ;
    rdfs:label "unranked" ;
    :isDefinedIn :core-conference-ranking ;
    rdfs:comment "The CORE category for a conference for which no ranking decision has been made." ;
    rdfs:isDefinedBy <http://purl.org/spar/bido-review-measures> .

:isLowerThan a owl:ObjectProperty ;
    rdfs:label "is lower than" ;
    rdfs:comment "It links a ranking category with one that is more important." ;
    rdfs:isDefinedBy <http://purl.org/spar/bido-review-measures> .

skos:inScheme a owl:ObjectProperty ;
    rdfs:isDefinedBy <http://www.w3.org/2004/02/skos/core> .

:DiscreteReviewerConfidenceScale a owl:Class ;
    rdfs:label "discrete reviewer confidence scale"@en ;
    rdfs:comment "A discrete scale defining the confidence of a reviewer for a given topic."@en ;
    rdfs:isDefinedBy <http://purl.org/spar/bido-review-measures> ;
    rdfs:subClassOf :ReviewerConfidenceScale .

:ScholarlyVenueManagementSystem a owl:Class ;
    rdfs:label "scholarly venue management system" ;
    rdfs:comment "This class describes all the possible venue management systems (such as conference management systems and journal management systems) that can be used for managing scholarly venues." ;
    rdfs:isDefinedBy <http://purl.org/spar/bido-review-measures> ;
    rdfs:subClassOf [ a owl:Restriction ;
            owl:allValuesFrom [ a owl:Restriction ;
                    owl:allValuesFrom [ a owl:Class ;
                            owl:unionOf ( swc:AcademicEvent fabio:Expression ) ] ;
                    owl:onProperty [ owl:inverseOf :holdsBibliometricDataInTime ] ] ;
            owl:onProperty [ owl:inverseOf :withBibliometricData ] ],
        :CategorialBibliometricData .

:acl-1-5-acl1 a :ReviewerConfidenceValue,
        owl:NamedIndividual ;
    rdfs:label "1 out of 5 (Discrete 1 to 5 review rating scale)"@en ;
    :hasConfidenceValue "1"^^xsd:int ;
    rdfs:comment "Not reviewer's area of expertise, or paper is very hard to understand. The evaluation is just an educated guess."@en ;
    rdfs:isDefinedBy <http://purl.org/spar/bido-review-measures> ;
    skos:closeMatch :acl-1-5-acl1,
        :ex-null-null ;
    skos:inScheme :acl-1-5 .

:acl-1-5-acl2 a :ReviewerConfidenceValue,
        owl:NamedIndividual ;
    rdfs:label "2 out of 5 (Discrete 1 to 5 review rating scale)"@en ;
    :hasConfidenceValue "2"^^xsd:int ;
    rdfs:comment "Reviewers is willing to defend my evaluation, but it is fairly likely that he/she missed some details, didn't understand some central points, or can't be sure about the novelty of the work."@en ;
    rdfs:isDefinedBy <http://purl.org/spar/bido-review-measures> ;
    skos:closeMatch :acl-1-5-acl2,
        :ex-null-low ;
    skos:inScheme :acl-1-5 .

:acl-1-5-acl3 a :ReviewerConfidenceValue,
        owl:NamedIndividual ;
    rdfs:label "3 out of 5 (Discrete 1 to 5 review rating scale)"@en ;
    :hasConfidenceValue "3"^^xsd:int ;
    rdfs:comment "Reviewer is pretty sure, but there's a chance he/she missed something. Although she/he has a good feel for this area in general, she/he did not carefully check the paper's details, e.g., the math, experimental design, or novelty."@en ;
    rdfs:isDefinedBy <http://purl.org/spar/bido-review-measures> ;
    skos:closeMatch :acl-1-5-acl3,
        :ex-null-med ;
    skos:inScheme :acl-1-5 .

:acl-1-5-acl4 a :ReviewerConfidenceValue,
        owl:NamedIndividual ;
    rdfs:label "4 out of 5 (Discrete 1 to 5 review rating scale)"@en ;
    :hasConfidenceValue "4"^^xsd:int ;
    rdfs:comment "Reviewer is quite sure, tried to check the important points carefully. It's unlikely, though conceivable, that he/she missed something that should affect his/her ratings."@en ;
    rdfs:isDefinedBy <http://purl.org/spar/bido-review-measures> ;
    skos:closeMatch :acl-1-5-acl4,
        :ex-null-high ;
    skos:inScheme :acl-1-5 .

:acl-1-5-acl5 a :ReviewerConfidenceValue,
        owl:NamedIndividual ;
    rdfs:label "5 out of 5 (Discrete 1 to 5 review rating scale)"@en ;
    :hasConfidenceValue "5"^^xsd:int ;
    rdfs:comment "Reviewer is positive that the evaluation is correct, has read the paper very carefully and is familiar with related work."@en ;
    rdfs:isDefinedBy <http://purl.org/spar/bido-review-measures> ;
    skos:closeMatch :acl-1-5-acl5,
        :ex-null-exp ;
    skos:inScheme :acl-1-5 .

:dis-0-5-2 a :ReviewRatingValue,
        owl:NamedIndividual ;
    rdfs:label "2 out of 5 (Discrete 0 to 5 review rating scale)"@en ;
    :hasRatingValue "2"^^xsd:int ;
    rdfs:isDefinedBy <http://purl.org/spar/bido-review-measures> ;
    skos:closeMatch :sa-sr-bl-wrej,
        :sa-sr-nb-wrej ;
    skos:inScheme :dis-0-5 .

:ex-null-exp a :ReviewerConfidenceValue,
        owl:NamedIndividual ;
    rdfs:label "Expert (Expert to Null reviewer confidence scale)"@en ;
    :hasConfidenceValue "4"^^xsd:int ;
    rdfs:isDefinedBy <http://purl.org/spar/bido-review-measures> ;
    skos:closeMatch :acl-1-5-acl5,
        :ex-null-exp ;
    skos:inScheme :ex-null .

:ex-null-high a :ReviewerConfidenceValue,
        owl:NamedIndividual ;
    rdfs:label "High (Expert to Null reviewer confidence scale)"@en ;
    :hasConfidenceValue "3"^^xsd:int ;
    rdfs:isDefinedBy <http://purl.org/spar/bido-review-measures> ;
    skos:closeMatch :acl-1-5-acl4,
        :ex-null-high ;
    skos:inScheme :ex-null .

:ex-null-low a :ReviewerConfidenceValue,
        owl:NamedIndividual ;
    rdfs:label "Low (Expert to Null reviewer confidence scale)"@en ;
    :hasConfidenceValue "1"^^xsd:int ;
    rdfs:isDefinedBy <http://purl.org/spar/bido-review-measures> ;
    skos:closeMatch :acl-1-5-acl2,
        :ex-null-low ;
    skos:inScheme :ex-null .

:ex-null-med a :ReviewerConfidenceValue,
        owl:NamedIndividual ;
    rdfs:label "Medium (Expert to Null reviewer confidence scale)"@en ;
    :hasConfidenceValue "2"^^xsd:int ;
    rdfs:isDefinedBy <http://purl.org/spar/bido-review-measures> ;
    skos:closeMatch :acl-1-5-acl3,
        :ex-null-med ;
    skos:inScheme :ex-null .

:ex-null-null a :ReviewerConfidenceValue,
        owl:NamedIndividual ;
    rdfs:label "Null (Expert to Null reviewer confidence scale)"@en ;
    :hasConfidenceValue "0"^^xsd:int ;
    rdfs:isDefinedBy <http://purl.org/spar/bido-review-measures> ;
    skos:closeMatch :acl-1-5-acl1,
        :ex-null-null ;
    skos:inScheme :ex-null .

:sa-sr-bl-wrej a :ReviewRatingValue,
        owl:NamedIndividual ;
    rdfs:label "Weak Reject (Strong Reject to Strong Accept review rating scale)"@en ;
    rdfs:isDefinedBy <http://purl.org/spar/bido-review-measures> ;
    skos:closeMatch :dis-0-5-2,
        :sa-sr-nb-wrej ;
    skos:inScheme :sa-sr-bl .

:sa-sr-nb-wrej a :ReviewRatingValue,
        owl:NamedIndividual ;
    rdfs:label "Weak Reject (Strong Reject to Strong Accept, without Borderline review rating scale)"@en ;
    rdfs:isDefinedBy <http://purl.org/spar/bido-review-measures> ;
    skos:closeMatch :dis-0-5-2,
        :sa-sr-bl-wrej ;
    skos:inScheme :sa-sr-nb .

:PeerReviewType a owl:Class ;
    rdfs:label "peer review type" ;
    rdfs:comment "This class describes different kinds of peer review processes, such as double-blind and open." ;
    rdfs:isDefinedBy <http://purl.org/spar/bido-review-measures> ;
    rdfs:subClassOf [ a owl:Restriction ;
            owl:allValuesFrom [ a owl:Restriction ;
                    owl:allValuesFrom [ a owl:Class ;
                            owl:unionOf ( swc:AcademicEvent fabio:Expression ) ] ;
                    owl:onProperty [ owl:inverseOf :holdsBibliometricDataInTime ] ] ;
            owl:onProperty [ owl:inverseOf :withBibliometricData ] ],
        :CategorialBibliometricData .

:a-na-wr a :DiscreteReviewRatingScale,
        owl:NamedIndividual ;
    rdfs:label "Approved to Not Approved review rating scale"@en ;
    rdfs:comment "Discrete scale from Approved to Not Approved, including Aprproved With Reservations."@en ;
    rdfs:isDefinedBy <http://purl.org/spar/bido-review-measures> .

:a-r-ts-majrev a :ReviewRatingValue,
        owl:NamedIndividual ;
    rdfs:label "Major revision (Accept to Reject, Two Strikes review rating scale)"@en ;
    rdfs:isDefinedBy <http://purl.org/spar/bido-review-measures> ;
    skos:closeMatch :dis-0-10-5,
        :dis-n2-p2-0,
        :sa-sr-bl-bdl ;
    skos:inScheme :a-r-ts .

:dis-0-10-5 a :ReviewRatingValue,
        owl:NamedIndividual ;
    rdfs:label "5 out of 10 (Discrete 0 to 10 review rating scale)"@en ;
    :hasRatingValue "5"^^xsd:int ;
    rdfs:isDefinedBy <http://purl.org/spar/bido-review-measures> ;
    skos:closeMatch :a-r-ts-majrev,
        :dis-n2-p2-0,
        :sa-sr-bl-bdl ;
    skos:inScheme :dis-0-10 .

:dis-n2-p2-0 a :ReviewRatingValue,
        owl:NamedIndividual ;
    rdfs:label "0 on a [-2,2] scale (Discrete -2 to 2 review rating scale)"@en ;
    :hasRatingValue "0"^^xsd:int ;
    rdfs:isDefinedBy <http://purl.org/spar/bido-review-measures> ;
    skos:closeMatch :a-r-ts-majrev,
        :dis-0-10-5,
        :sa-sr-bl-bdl ;
    skos:inScheme :dis-n2-p2 .

:sa-sr-bl-bdl a :ReviewRatingValue,
        owl:NamedIndividual ;
    rdfs:label "Borderline (Strong Reject to Strong Accept review rating scale)"@en ;
    rdfs:isDefinedBy <http://purl.org/spar/bido-review-measures> ;
    skos:closeMatch :a-r-ts-majrev,
        :dis-0-10-5,
        :dis-n2-p2-0 ;
    skos:inScheme :sa-sr-bl .

:ReviewRatingScale a owl:Class ;
    rdfs:label "review rating scale"@en ;
    rdfs:comment "A scale defining the rating given by a reviewer for a specific scientific contribution."@en ;
    rdfs:isDefinedBy <http://purl.org/spar/bido-review-measures> ;
    rdfs:subClassOf skos:ConceptScheme .

:a-na-wr-appwr a :ReviewRatingValue,
        owl:NamedIndividual ;
    rdfs:label "Approved with reservations (Approved to Not Approved review rating scale)"@en ;
    rdfs:isDefinedBy <http://purl.org/spar/bido-review-measures> ;
    skos:closeMatch :a-r-ts-minrev,
        :dis-0-5-3,
        :sa-sr-bl-wacc,
        :sa-sr-nb-wacc ;
    skos:inScheme :a-na-wr .

:a-r-ts-minrev a :ReviewRatingValue,
        owl:NamedIndividual ;
    rdfs:label "Minor revision (Accept to Reject, Two Strikes review rating scale)"@en ;
    rdfs:isDefinedBy <http://purl.org/spar/bido-review-measures> ;
    skos:closeMatch :a-na-wr-appwr,
        :dis-0-5-3,
        :sa-sr-bl-wacc,
        :sa-sr-nb-wacc ;
    skos:inScheme :a-r-ts .

:dis-0-5-3 a :ReviewRatingValue,
        owl:NamedIndividual ;
    rdfs:label "3 out of 5 (Discrete 0 to 5 review rating scale)"@en ;
    :hasRatingValue "3"^^xsd:int ;
    rdfs:isDefinedBy <http://purl.org/spar/bido-review-measures> ;
    skos:closeMatch :a-na-wr-appwr,
        :a-r-ts-minrev,
        :sa-sr-bl-wacc,
        :sa-sr-nb-wacc ;
    skos:inScheme :dis-0-5 .

:sa-sr-bl-wacc a :ReviewRatingValue,
        owl:NamedIndividual ;
    rdfs:label "Weak Accept (Strong Reject to Strong Accept review rating scale)"@en ;
    rdfs:isDefinedBy <http://purl.org/spar/bido-review-measures> ;
    skos:closeMatch :a-na-wr-appwr,
        :a-r-ts-minrev,
        :dis-0-5-3,
        :sa-sr-nb-wacc ;
    skos:inScheme :sa-sr-bl .

:sa-sr-nb-wacc a :ReviewRatingValue,
        owl:NamedIndividual ;
    rdfs:label "Weak Accept (Strong Reject to Strong Accept, without Borderline review rating scale)"@en ;
    rdfs:isDefinedBy <http://purl.org/spar/bido-review-measures> ;
    skos:closeMatch :a-na-wr-appwr,
        :a-r-ts-minrev,
        :dis-0-5-3,
        :sa-sr-bl-wacc ;
    skos:inScheme :sa-sr-nb .

skos:ConceptScheme a owl:Class ;
    rdfs:isDefinedBy <http://www.w3.org/2004/02/skos/core> .

:ConferenceRankingCategory a owl:Class ;
    rdfs:label "conference ranking category" ;
    rdfs:comment "This class identifies all the possible categories that can be used for ranking a conference according to the related ranking that defines them." ;
    rdfs:isDefinedBy <http://purl.org/spar/bido-review-measures> ;
    rdfs:subClassOf [ a owl:Restriction ;
            owl:allValuesFrom [ a owl:Restriction ;
                    owl:allValuesFrom swc:AcademicEvent ;
                    owl:onProperty [ owl:inverseOf :holdsBibliometricDataInTime ] ] ;
            owl:onProperty [ owl:inverseOf :withBibliometricData ] ],
        :CategorialBibliometricData .

:acl-1-5 a :DiscreteReviewerConfidenceScale,
        owl:NamedIndividual ;
    rdfs:label "Discrete 1 to 5 review rating scale"@en ;
    rdfs:comment "Discrete scale from 1 to 5, used by Association for Computational Linguistics annual meetings"@en ;
    rdfs:isDefinedBy <http://purl.org/spar/bido-review-measures> .

:core-conference-ranking a :ConferenceRanking,
        owl:NamedIndividual ;
    rdfs:label "CORE conference ranking" ;
    rdfs:comment "The CORE Conference Ranking (http://www.core.edu.au/index.php/conference-rankings) is an ongoing activity that provides assessments of major conferences in the computing disciplines.The rankings are managed by the CORE Executive Committee, with updates processed from time to time by a subcommittee established as needed." ;
    rdfs:isDefinedBy <http://purl.org/spar/bido-review-measures> .

:dis-0-5-1 a :ReviewRatingValue,
        owl:NamedIndividual ;
    rdfs:label "1 out of 5 (Discrete 0 to 5 review rating scale)"@en ;
    :hasRatingValue "1"^^xsd:int ;
    rdfs:isDefinedBy <http://purl.org/spar/bido-review-measures> ;
    skos:closeMatch :a-na-wr-napp,
        :a-r-ts-rej,
        :dis-n2-p2-neg1,
        :sa-sr-bl-rej,
        :sa-sr-nb-rej ;
    skos:inScheme :dis-0-5 .

:dis-0-5-4 a :ReviewRatingValue,
        owl:NamedIndividual ;
    rdfs:label "4 out of 5 (Discrete 0 to 5 review rating scale)"@en ;
    :hasRatingValue "4"^^xsd:int ;
    rdfs:isDefinedBy <http://purl.org/spar/bido-review-measures> ;
    skos:closeMatch :a-na-wr-app,
        :a-r-ts-acc,
        :dis-n2-p2-pos1,
        :sa-sr-bl-acc,
        :sa-sr-nb-acc ;
    skos:inScheme :dis-0-5 .

:dis-n2-p2 a :DiscreteReviewRatingScale,
        owl:NamedIndividual ;
    rdfs:label "Discrete -2 to 2 review rating scale"@en ;
    rdfs:comment "Discrete scale from -2 to 2, including 0"@en ;
    rdfs:isDefinedBy <http://purl.org/spar/bido-review-measures> .

:dis-n2-p2-neg1 a :ReviewRatingValue,
        owl:NamedIndividual ;
    rdfs:label "-1 on a [-2,2] scale (Discrete -2 to 2 review rating scale)"@en ;
    :hasRatingValue "-1"^^xsd:int ;
    rdfs:isDefinedBy <http://purl.org/spar/bido-review-measures> ;
    skos:closeMatch :a-na-wr-napp,
        :a-r-ts-rej,
        :dis-0-5-1,
        :sa-sr-bl-rej,
        :sa-sr-nb-rej ;
    skos:inScheme :dis-n2-p2 .

:dis-n2-p2-pos1 a :ReviewRatingValue,
        owl:NamedIndividual ;
    rdfs:label "1 on a [-2,2] scale (Discrete -2 to 2 review rating scale)"@en ;
    :hasRatingValue "1"^^xsd:int ;
    rdfs:isDefinedBy <http://purl.org/spar/bido-review-measures> ;
    skos:closeMatch :a-na-wr-app,
        :a-r-ts-acc,
        :dis-0-5-4,
        :sa-sr-bl-acc,
        :sa-sr-nb-acc ;
    skos:inScheme :dis-n2-p2 .

:ex-null a :DiscreteReviewerConfidenceScale,
        owl:NamedIndividual ;
    rdfs:label "Expert to Null reviewer confidence scale"@en ;
    rdfs:comment "Discrete scale from Expert to Null, also representend in an scale from 4 to 0"@en ;
    rdfs:isDefinedBy <http://purl.org/spar/bido-review-measures> .

:sa-sr-bl-acc a :ReviewRatingValue,
        owl:NamedIndividual ;
    rdfs:label "Accept (Strong Reject to Strong Accept review rating scale)"@en ;
    rdfs:isDefinedBy <http://purl.org/spar/bido-review-measures> ;
    skos:closeMatch :a-na-wr-app,
        :a-r-ts-acc,
        :dis-0-5-4,
        :dis-n2-p2-pos1,
        :sa-sr-nb-acc ;
    skos:inScheme :sa-sr-bl .

:sa-sr-bl-rej a :ReviewRatingValue,
        owl:NamedIndividual ;
    rdfs:label "Reject (Strong Reject to Strong Accept review rating scale)"@en ;
    rdfs:isDefinedBy <http://purl.org/spar/bido-review-measures> ;
    skos:closeMatch :a-na-wr-napp,
        :a-r-ts-rej,
        :dis-0-5-1,
        :dis-n2-p2-neg1,
        :sa-sr-nb-rej ;
    skos:inScheme :sa-sr-bl .

:sa-sr-nb-acc a :ReviewRatingValue,
        owl:NamedIndividual ;
    rdfs:label "Accept (Strong Reject to Strong Accept, without Borderline review rating scale)"@en ;
    rdfs:isDefinedBy <http://purl.org/spar/bido-review-measures> ;
    skos:closeMatch :a-na-wr-app,
        :a-r-ts-acc,
        :dis-0-10-10,
        :dis-0-5-4,
        :dis-n2-p2-pos1,
        :sa-sr-bl-acc ;
    skos:inScheme :sa-sr-nb .

:sa-sr-nb-rej a :ReviewRatingValue,
        owl:NamedIndividual ;
    rdfs:label "Reject (Strong Reject to Strong Accept, without Borderline review rating scale)"@en ;
    rdfs:isDefinedBy <http://purl.org/spar/bido-review-measures> ;
    skos:closeMatch :a-na-wr-napp,
        :a-r-ts-rej,
        :dis-0-10-0,
        :dis-0-5-1,
        :dis-n2-p2-neg1,
        :sa-sr-bl-rej ;
    skos:inScheme :sa-sr-nb .

:a-r-ts a :DiscreteReviewRatingScale,
        owl:NamedIndividual ;
    rdfs:label "Accept to Reject, Two Strikes review rating scale"@en ;
    rdfs:comment "Discrete scale from Accept to Reject, including pre-screening and two strikes rule"@en ;
    rdfs:isDefinedBy <http://purl.org/spar/bido-review-measures> .

:dis-0-5 a :DiscreteReviewRatingScale,
        owl:NamedIndividual ;
    rdfs:label "Discrete 0 to 5 review rating scale"@en ;
    rdfs:comment "Discrete scale from 0 to 5"@en ;
    rdfs:isDefinedBy <http://purl.org/spar/bido-review-measures> .

:dis-0-5-0 a :ReviewRatingValue,
        owl:NamedIndividual ;
    rdfs:label "0 out of 5 (Discrete 0 to 5 review rating scale)"@en ;
    :hasRatingValue "0"^^xsd:int ;
    rdfs:isDefinedBy <http://purl.org/spar/bido-review-measures> ;
    skos:closeMatch :a-na-wr-napp,
        :a-r-ts-rej,
        :dis-0-10-0,
        :dis-n2-p2-neg2,
        :sa-sr-bl-srej,
        :sa-sr-nb-srej ;
    skos:inScheme :dis-0-5 .

:dis-0-5-5 a :ReviewRatingValue,
        owl:NamedIndividual ;
    rdfs:label "5 out of 5 (Discrete 0 to 5 review rating scale)"@en ;
    :hasRatingValue "5"^^xsd:int ;
    rdfs:isDefinedBy <http://purl.org/spar/bido-review-measures> ;
    skos:closeMatch :a-na-wr-app,
        :a-r-ts-acc,
        :dis-0-10-10,
        :dis-n2-p2-pos2,
        :sa-sr-bl-sacc,
        :sa-sr-nb-sacc ;
    skos:inScheme :dis-0-5 .

:dis-n2-p2-neg2 a :ReviewRatingValue,
        owl:NamedIndividual ;
    rdfs:label "-2 on a [-2,2] scale (Discrete -2 to 2 review rating scale)"@en ;
    :hasRatingValue "-2"^^xsd:int ;
    rdfs:isDefinedBy <http://purl.org/spar/bido-review-measures> ;
    skos:closeMatch :a-na-wr-napp,
        :a-r-ts-rej,
        :dis-0-10-0,
        :dis-0-5-0,
        :sa-sr-bl-srej,
        :sa-sr-nb-srej ;
    skos:inScheme :dis-n2-p2 .

:dis-n2-p2-pos2 a :ReviewRatingValue,
        owl:NamedIndividual ;
    rdfs:label "2 on a [-2,2] scale (Discrete -2 to 2 review rating scale)"@en ;
    :hasRatingValue "2"^^xsd:int ;
    rdfs:isDefinedBy <http://purl.org/spar/bido-review-measures> ;
    skos:closeMatch :a-na-wr-app,
        :a-r-ts-acc,
        :dis-0-10-10,
        :dis-0-5-5,
        :sa-sr-bl-sacc,
        :sa-sr-nb-sacc ;
    skos:inScheme :dis-n2-p2 .

:sa-sr-bl-sacc a :ReviewRatingValue,
        owl:NamedIndividual ;
    rdfs:label "Strong Accept (Strong Reject to Strong Accept review rating scale)"@en ;
    rdfs:isDefinedBy <http://purl.org/spar/bido-review-measures> ;
    skos:closeMatch :a-na-wr-app,
        :a-r-ts-acc,
        :dis-0-10-10,
        :dis-0-5-5,
        :dis-n2-p2-pos2,
        :sa-sr-nb-sacc ;
    skos:inScheme :sa-sr-bl .

:sa-sr-bl-srej a :ReviewRatingValue,
        owl:NamedIndividual ;
    rdfs:label "Strong Reject (Strong Reject to Strong Accept review rating scale)"@en ;
    rdfs:isDefinedBy <http://purl.org/spar/bido-review-measures> ;
    skos:closeMatch :a-na-wr-napp,
        :a-r-ts-rej,
        :dis-0-10-0,
        :dis-0-5-0,
        :dis-n2-p2-neg2,
        :sa-sr-nb-srej ;
    skos:inScheme :sa-sr-bl .

:sa-sr-nb a :DiscreteReviewRatingScale,
        owl:NamedIndividual ;
    rdfs:label "Strong Reject to Strong Accept, without Borderline review rating scale"@en ;
    rdfs:comment "Discrete scale from Strong Reject to Strong Accept, excluding Bordeline"@en ;
    rdfs:isDefinedBy <http://purl.org/spar/bido-review-measures> .

:sa-sr-nb-sacc a :ReviewRatingValue,
        owl:NamedIndividual ;
    rdfs:label "Strong Accept (Strong Reject to Strong Accept, without Borderline review rating scale)"@en ;
    rdfs:isDefinedBy <http://purl.org/spar/bido-review-measures> ;
    skos:closeMatch :a-na-wr-app,
        :a-r-ts-acc,
        :dis-0-10-10,
        :dis-0-5-5,
        :dis-n2-p2-pos2,
        :sa-sr-bl-sacc ;
    skos:inScheme :sa-sr-nb .

:sa-sr-nb-srej a :ReviewRatingValue,
        owl:NamedIndividual ;
    rdfs:label "Strong Reject (Strong Reject to Strong Accept, without Borderline review rating scale)"@en ;
    rdfs:isDefinedBy <http://purl.org/spar/bido-review-measures> ;
    skos:closeMatch :a-na-wr-napp,
        :a-r-ts-rej,
        :dis-0-10-0,
        :dis-0-5-0,
        :dis-n2-p2-neg2,
        :sa-sr-bl-srej ;
    skos:inScheme :sa-sr-nb .

:BibliometricMeasure a owl:Class .

:DiscreteReviewRatingScale a owl:Class ;
    rdfs:label "discrete review rating scale"@en ;
    rdfs:comment "A discrete scale defining the rating given by a reviewer for a specific scientific contribution."@en ;
    rdfs:isDefinedBy <http://purl.org/spar/bido-review-measures> ;
    rdfs:subClassOf :ReviewRatingScale .

:dis-0-10-0 a :ReviewRatingValue,
        owl:NamedIndividual ;
    rdfs:label "0 out of 10 (Discrete 0 to 10 review rating scale)"@en ;
    :hasRatingValue "0"^^xsd:int ;
    rdfs:isDefinedBy <http://purl.org/spar/bido-review-measures> ;
    skos:closeMatch :a-na-wr-napp,
        :a-r-ts-rej,
        :dis-0-5-0,
        :dis-n2-p2-neg2,
        :sa-sr-bl-srej,
        :sa-sr-nb-srej ;
    skos:inScheme :dis-0-10 .

:dis-0-10-10 a :ReviewRatingValue,
        owl:NamedIndividual ;
    rdfs:label "10 out of 10 (Discrete 0 to 10 review rating scale)"@en ;
    :hasRatingValue "10"^^xsd:int ;
    rdfs:isDefinedBy <http://purl.org/spar/bido-review-measures> ;
    skos:closeMatch :a-na-wr-app,
        :a-r-ts-acc,
        :dis-0-5-5,
        :dis-n2-p2-pos2,
        :sa-sr-bl-sacc,
        :sa-sr-nb-sacc ;
    skos:inScheme :dis-0-10 .

:hasMeasure a owl:ObjectProperty .

:sa-sr-bl a :DiscreteReviewRatingScale,
        owl:NamedIndividual ;
    rdfs:label "Strong Reject to Strong Accept review rating scale"@en ;
    rdfs:comment "Discrete scale from Strong Reject to Strong Accept, including Bordeline"@en ;
    rdfs:isDefinedBy <http://purl.org/spar/bido-review-measures> .

:CategorialBibliometricData a owl:Class .

fabio:Expression a owl:Class ;
    rdfs:label "expression" ;
    rdfs:comment "Any possible work such as journals, magazines, books, etc., created for scientific purposes and possibily related with review processes." ;
    rdfs:isDefinedBy <http://purl.org/spar/fabio> .

swc:AcademicEvent a owl:Class ;
    rdfs:label "academic event" ;
    rdfs:comment "Any academic event such as conferences, workshops, symposia." ;
    rdfs:isDefinedBy <http://data.semanticweb.org/ns/swc/ontology> .

:a-na-wr-app a :ReviewRatingValue,
        owl:NamedIndividual ;
    rdfs:label "Approved (Approved to Not Approved review rating scale)"@en ;
    rdfs:isDefinedBy <http://purl.org/spar/bido-review-measures> ;
    skos:closeMatch :a-r-ts-acc,
        :dis-0-10-10,
        :dis-0-5-4,
        :dis-0-5-5,
        :dis-n2-p2-pos1,
        :dis-n2-p2-pos2,
        :sa-sr-bl-acc,
        :sa-sr-bl-sacc,
        :sa-sr-nb-acc,
        :sa-sr-nb-sacc ;
    skos:inScheme :a-na-wr .

:a-na-wr-napp a :ReviewRatingValue,
        owl:NamedIndividual ;
    rdfs:label "Not approved (Approved to Not Approved review rating scale)"@en ;
    rdfs:isDefinedBy <http://purl.org/spar/bido-review-measures> ;
    skos:closeMatch :a-r-ts-rej,
        :dis-0-10-0,
        :dis-0-5-0,
        :dis-0-5-1,
        :dis-n2-p2-neg1,
        :dis-n2-p2-neg2,
        :sa-sr-bl-rej,
        :sa-sr-bl-srej,
        :sa-sr-nb-rej,
        :sa-sr-nb-srej ;
    skos:inScheme :a-na-wr .

:a-r-ts-acc a :ReviewRatingValue,
        owl:NamedIndividual ;
    rdfs:label "Accept (Accept to Reject, Two Strikes review rating scale)"@en ;
    rdfs:isDefinedBy <http://purl.org/spar/bido-review-measures> ;
    skos:closeMatch :a-na-wr-app,
        :dis-0-10-10,
        :dis-0-5-4,
        :dis-0-5-5,
        :dis-n2-p2-pos1,
        :dis-n2-p2-pos2,
        :sa-sr-bl-acc,
        :sa-sr-bl-sacc,
        :sa-sr-nb-acc,
        :sa-sr-nb-sacc ;
    skos:inScheme :a-r-ts .

:a-r-ts-rej a :ReviewRatingValue,
        owl:NamedIndividual ;
    rdfs:label "Reject (Accept to Reject, Two Strikes review rating scale)"@en ;
    rdfs:isDefinedBy <http://purl.org/spar/bido-review-measures> ;
    skos:closeMatch :a-na-wr-napp,
        :dis-0-10-0,
        :dis-0-5-0,
        :dis-0-5-1,
        :dis-n2-p2-neg1,
        :dis-n2-p2-neg2,
        :sa-sr-bl-rej,
        :sa-sr-bl-srej,
        :sa-sr-nb-rej,
        :sa-sr-nb-srej ;
    skos:inScheme :a-r-ts .

:holdsBibliometricDataInTime a owl:ObjectProperty .

:withBibliometricData a owl:ObjectProperty .

:ReviewerConfidenceValue a owl:Class ;
    rdfs:label "reviewer confidence value"@en ;
    rdfs:comment "This class describes the set of values compliant with a given reviewer confidence scale."@en ;
    rdfs:isDefinedBy <http://purl.org/spar/bido-review-measures> ;
    rdfs:subClassOf :CategorialBibliometricData .

:dis-0-10 a :DiscreteReviewRatingScale,
        owl:NamedIndividual ;
    rdfs:label "Discrete 0 to 10 review rating scale"@en ;
    rdfs:comment "Discrete scale from 0 to 10"@en ;
    rdfs:isDefinedBy <http://purl.org/spar/bido-review-measures> .

:ReviewRatingValue a owl:Class ;
    rdfs:label "review rating value"@en ;
    rdfs:comment "This class describes the set of values compliant with a given review rating scale."@en ;
    rdfs:isDefinedBy <http://purl.org/spar/bido-review-measures> ;
    rdfs:subClassOf :CategorialBibliometricData .

<http://purl.org/spar/bido-review-measures> a owl:Ontology ;
    rdfs:label "BiDO-Review-Measures" ;
    dc:contributor "Aliaksandr Birukou" ;
    dc:creator "Idafen Santana-Pérez",
        "María Poveda-Villalón",
        "Silvio Peroni" ;
    dc:date "2018-07-13"^^xsd:string ;
    dc:description """The need of describing aspects related to the review process is an important aspect to address by publishers (e.g., Springer) for keeping track of crucial information about conferences and journals. In addition, these data can be crucial for assessing the quality of the venues where researchers publish papers.

This module of BiDO describes a list of possible reviews measures tha can be used to define bibliometric data of scholarly venues such as conferences, workshops, and journals.""" ;
    dc:rights "This work is distributed under a Creative Commons Attribution License (http://creativecommons.org/licenses/by/4.0/)." ;
    dc:title "BiDO Review Measures module (BiDO-Review-Measures)" ;
    rdfs:comment """The BiDO Review Measures module (BiDO-Review-Measures) describes a list of possible reviews measures that can be used to define bibliometric data of scholarly venues such as conferences, workshops, journals.

**URL:** http://purl.org/spar/bido-review-measures

**Creators**: [Silvio Peroni](http://orcid.org/0000-0003-0530-4305), [Idafen Santana-Pérez](https://orcid.org/0000-0001-8296-8629), [María Poveda-Villalón](https://orcid.org/0000-0003-3587-0367)

**Contributors**: [Aliaksandr Birukou](https://orcid.org/0000-0002-4925-9131)

**License:** [Creative Commons Attribution 4.0 International](https://creativecommons.org/licenses/by/4.0/legalcode)

**Website:** http://www.sparontologies.net/ontologies/bido"""^^xsd:string ;
    owl:imports <http://purl.org/spar/bido-core> ;
    owl:priorVersion <http://purl.org/spar/bido-review-measures/2015-07-13> ;
    owl:versionIRI <http://purl.org/spar/bido-review-measures/2018-07-13> ;
    owl:versionInfo "1.1"^^xsd:string .

