@prefix : <http://purl.org/spar/bido/> .
@prefix dc: <http://purl.org/dc/elements/1.1/> .
@prefix owl: <http://www.w3.org/2002/07/owl#> .
@prefix rdf: <http://www.w3.org/1999/02/22-rdf-syntax-ns#> .
@prefix swc: <http://data.semanticweb.org/ns/swc/ontology#> .
@prefix xml: <http://www.w3.org/XML/1998/namespace> .
@prefix xsd: <http://www.w3.org/2001/XMLSchema#> .
@prefix rdfs: <http://www.w3.org/2000/01/rdf-schema#> .
@prefix fabio: <http://purl.org/spar/fabio/> .

<http://purl.org/spar/bido-review-measures> a owl:Ontology ;
	owl:versionIRI <http://purl.org/spar/bido-review-measures/2018-07-13> ;
	owl:imports <http://purl.org/spar/bido-core> ;
	dc:creator "Idafen Santana-Pérez" ;
	dc:title "BiDO Review Measures module (BiDO-Review-Measures)" ;
	dc:creator "Silvio Peroni" , "María Poveda-Villalón" ;
	owl:versionInfo "1.1"^^xsd:string ;
	dc:rights "This work is distributed under a Creative Commons Attribution License (http://creativecommons.org/licenses/by/4.0/)." ;
	rdfs:label "BiDO-Review-Measures" ;
	rdfs:comment """The BiDO Review Measures module (BiDO-Review-Measures) describes a list of possible reviews measures that can be used to define bibliometric data of scholarly venues such as conferences, workshops, journals.

**URL:** http://purl.org/spar/bido-review-measures

**Creators**: [Silvio Peroni](http://orcid.org/0000-0003-0530-4305), [Idafen Santana-Pérez](https://orcid.org/0000-0001-8296-8629), [María Poveda-Villalón](https://orcid.org/0000-0003-3587-0367)

**Contributors**: [Aliaksandr Birukou](https://orcid.org/0000-0002-4925-9131)

**License:** [Creative Commons Attribution 4.0 International](https://creativecommons.org/licenses/by/4.0/legalcode)

**Website:** http://www.sparontologies.net/ontologies/bido"""^^xsd:string ;
	dc:date "2018-07-13"^^xsd:string ;
	dc:description """The need of describing aspects related to the review process is an important aspect to address by publishers (e.g., Springer) for keeping track of crucial information about conferences and journals. In addition, these data can be crucial for assessing the quality of the venues where researchers publish papers.

This module of BiDO describes a list of possible reviews measures tha can be used to define bibliometric data of scholarly venues such as conferences, workshops, and journals.""" ;
	dc:contributor "Aliaksandr Birukou" ;
	owl:priorVersion <http://purl.org/spar/bido-review-measures/2015-07-13> .
# 
# 
# #################################################################
# #
# #    Object Properties
# #
# #################################################################
# 
# 
# http://purl.org/spar/bido/isDefinedIn

:isDefinedIn a owl:ObjectProperty ;
	rdfs:subPropertyOf <http://www.w3.org/2004/02/skos/core#inScheme> ;
	rdfs:domain :CategorialBibliometricData ;
	rdfs:range <http://www.w3.org/2004/02/skos/core#ConceptScheme> ;
	rdfs:comment "It links a ranking category with the ranking that defines it." ;
	rdfs:isDefinedBy <http://purl.org/spar/bido-review-measures> ;
	rdfs:label "is defined in ranking" .
# 
# http://purl.org/spar/bido/isHigherThan

:isHigherThan a owl:ObjectProperty ;
	owl:inverseOf :isLowerThan ;
	rdfs:domain :CategorialBibliometricData ;
	rdfs:range :CategorialBibliometricData ;
	rdfs:comment "It links a ranking category with one that is less important." ;
	rdfs:isDefinedBy <http://purl.org/spar/bido-review-measures> ;
	rdfs:label "is higher than" .
# 
# http://purl.org/spar/bido/isLowerThan

:isLowerThan a owl:ObjectProperty ;
	rdfs:comment "It links a ranking category with one that is more important." ;
	rdfs:isDefinedBy <http://purl.org/spar/bido-review-measures> ;
	rdfs:label "is lower than" .
# 
# http://www.w3.org/2004/02/skos/core#closeMatch

<http://www.w3.org/2004/02/skos/core#closeMatch> a owl:ObjectProperty ;
	rdfs:isDefinedBy <http://www.w3.org/2004/02/skos/core> .
# 
# http://www.w3.org/2004/02/skos/core#inScheme

<http://www.w3.org/2004/02/skos/core#inScheme> a owl:ObjectProperty ;
	rdfs:isDefinedBy <http://www.w3.org/2004/02/skos/core> .
# 
# 
# 
# #################################################################
# #
# #    Data properties
# #
# #################################################################
# 
# 
# http://purl.org/spar/bido/hasConfidenceValue

:hasConfidenceValue a owl:DatatypeProperty ;
	rdfs:domain :ReviewerConfidenceValue ;
	rdfs:range rdfs:Literal ;
	rdfs:comment "The confidence value of expertise in the review topic given by the reviwer."@en ;
	rdfs:isDefinedBy <http://purl.org/spar/bido-review-measures> ;
	rdfs:label "has confidence value"@en .
# 
# http://purl.org/spar/bido/hasRatingValue

:hasRatingValue a owl:DatatypeProperty ;
	rdfs:domain :ReviewRatingValue ;
	rdfs:range rdfs:Literal ;
	rdfs:comment "The value of the rating given to a review."@en ;
	rdfs:isDefinedBy <http://purl.org/spar/bido-review-measures> ;
	rdfs:label "has rating value"@en .
# 
# 
# 
# #################################################################
# #
# #    Classes
# #
# #################################################################
# 
# 
# http://data.semanticweb.org/ns/swc/ontology#AcademicEvent

swc:AcademicEvent a owl:Class ;
	rdfs:comment "Any academic event such as conferences, workshops, symposia." ;
	rdfs:isDefinedBy <http://data.semanticweb.org/ns/swc/ontology> ;
	rdfs:label "academic event" .
# 
# http://purl.org/spar/bido/ConferenceRanking

:ConferenceRanking a owl:Class ;
	rdfs:subClassOf <http://www.w3.org/2004/02/skos/core#ConceptScheme> ;
	rdfs:comment "This class describes conference rankings as composed by categories identifying different rankings." ;
	rdfs:isDefinedBy <http://purl.org/spar/bido-review-measures> ;
	rdfs:label "conference ranking" .
# 
# http://purl.org/spar/bido/ConferenceRankingCategory

:ConferenceRankingCategory a owl:Class ;
	rdfs:subClassOf :CategorialBibliometricData , _:genid1 .

_:genid1 a owl:Restriction ;
	owl:onProperty _:genid2 .

_:genid2 owl:inverseOf :withBibliometricData .

_:genid1 owl:allValuesFrom _:genid3 .

_:genid3 a owl:Restriction ;
	owl:onProperty _:genid4 .

_:genid4 owl:inverseOf :holdsBibliometricDataInTime .

_:genid3 owl:allValuesFrom swc:AcademicEvent .

:ConferenceRankingCategory rdfs:comment "This class identifies all the possible categories that can be used for ranking a conference according to the related ranking that defines them." ;
	rdfs:isDefinedBy <http://purl.org/spar/bido-review-measures> ;
	rdfs:label "conference ranking category" .
# 
# http://purl.org/spar/bido/DiscreteReviewRatingScale

:DiscreteReviewRatingScale a owl:Class ;
	rdfs:subClassOf :ReviewRatingScale ;
	rdfs:comment "A discrete scale defining the rating given by a reviewer for a specific scientific contribution."@en ;
	rdfs:isDefinedBy <http://purl.org/spar/bido-review-measures> ;
	rdfs:label "discrete review rating scale"@en .
# 
# http://purl.org/spar/bido/DiscreteReviewerConfidenceScale

:DiscreteReviewerConfidenceScale a owl:Class ;
	rdfs:subClassOf :ReviewerConfidenceScale ;
	rdfs:comment "A discrete scale defining the confidence of a reviewer for a given topic."@en ;
	rdfs:isDefinedBy <http://purl.org/spar/bido-review-measures> ;
	rdfs:label "discrete reviewer confidence scale"@en .
# 
# http://purl.org/spar/bido/PeerReviewType

:PeerReviewType a owl:Class ;
	rdfs:subClassOf :CategorialBibliometricData , _:genid5 .

_:genid5 a owl:Restriction ;
	owl:onProperty _:genid6 .

_:genid6 owl:inverseOf :withBibliometricData .

_:genid5 owl:allValuesFrom _:genid7 .

_:genid7 a owl:Restriction ;
	owl:onProperty _:genid8 .

_:genid8 owl:inverseOf :holdsBibliometricDataInTime .

_:genid7 owl:allValuesFrom _:genid9 .

_:genid9 a owl:Class ;
	owl:unionOf _:genid11 .

_:genid11 a rdf:List ;
	rdf:first swc:AcademicEvent ;
	rdf:rest _:genid10 .

_:genid10 a rdf:List ;
	rdf:first fabio:Expression ;
	rdf:rest rdf:nil .

:PeerReviewType rdfs:comment "This class describes different kinds of peer review processes, such as double-blind and open." ;
	rdfs:isDefinedBy <http://purl.org/spar/bido-review-measures> ;
	rdfs:label "peer review type" .
# 
# http://purl.org/spar/bido/ReviewRatingScale

:ReviewRatingScale a owl:Class ;
	rdfs:subClassOf <http://www.w3.org/2004/02/skos/core#ConceptScheme> ;
	rdfs:comment "A scale defining the rating given by a reviewer for a specific scientific contribution."@en ;
	rdfs:isDefinedBy <http://purl.org/spar/bido-review-measures> ;
	rdfs:label "review rating scale"@en .
# 
# http://purl.org/spar/bido/ReviewRatingValue

:ReviewRatingValue a owl:Class ;
	rdfs:subClassOf :CategorialBibliometricData ;
	rdfs:comment "This class describes the set of values compliant with a given review rating scale."@en ;
	rdfs:isDefinedBy <http://purl.org/spar/bido-review-measures> ;
	rdfs:label "review rating value"@en .
# 
# http://purl.org/spar/bido/ReviewerConfidenceScale

:ReviewerConfidenceScale a owl:Class ;
	rdfs:subClassOf <http://www.w3.org/2004/02/skos/core#ConceptScheme> ;
	rdfs:comment "A scale defining the confidence of a reviewer for a given topic."@en ;
	rdfs:isDefinedBy <http://purl.org/spar/bido-review-measures> ;
	rdfs:label "reviewer confidence scale"@en .
# 
# http://purl.org/spar/bido/ReviewerConfidenceValue

:ReviewerConfidenceValue a owl:Class ;
	rdfs:subClassOf :CategorialBibliometricData ;
	rdfs:comment "This class describes the set of values compliant with a given reviewer confidence scale."@en ;
	rdfs:isDefinedBy <http://purl.org/spar/bido-review-measures> ;
	rdfs:label "reviewer confidence value"@en .
# 
# http://purl.org/spar/bido/ScholarlyVenueManagementSystem

:ScholarlyVenueManagementSystem a owl:Class ;
	rdfs:subClassOf :CategorialBibliometricData , _:genid12 .

_:genid12 a owl:Restriction ;
	owl:onProperty _:genid13 .

_:genid13 owl:inverseOf :withBibliometricData .

_:genid12 owl:allValuesFrom _:genid14 .

_:genid14 a owl:Restriction ;
	owl:onProperty _:genid15 .

_:genid15 owl:inverseOf :holdsBibliometricDataInTime .

_:genid14 owl:allValuesFrom _:genid16 .

_:genid16 a owl:Class ;
	owl:unionOf _:genid18 .

_:genid18 a rdf:List ;
	rdf:first swc:AcademicEvent ;
	rdf:rest _:genid17 .

_:genid17 a rdf:List ;
	rdf:first fabio:Expression ;
	rdf:rest rdf:nil .

:ScholarlyVenueManagementSystem rdfs:comment "This class describes all the possible venue management systems (such as conference management systems and journal management systems) that can be used for managing scholarly venues." ;
	rdfs:isDefinedBy <http://purl.org/spar/bido-review-measures> ;
	rdfs:label "scholarly venue management system" .
# 
# http://purl.org/spar/fabio/Expression

fabio:Expression a owl:Class ;
	rdfs:comment "Any possible work such as journals, magazines, books, etc., created for scientific purposes and possibily related with review processes." ;
	rdfs:isDefinedBy <http://purl.org/spar/fabio> ;
	rdfs:label "expression" .
# 
# http://www.w3.org/2004/02/skos/core#ConceptScheme

<http://www.w3.org/2004/02/skos/core#ConceptScheme> a owl:Class ;
	rdfs:isDefinedBy <http://www.w3.org/2004/02/skos/core> .
# 
# 
# 
# #################################################################
# #
# #    Individuals
# #
# #################################################################
# 
# 
# http://purl.org/NET/rdflicense/cc-by4.0

<http://purl.org/NET/rdflicense/cc-by4.0> a owl:NamedIndividual .
# 
# http://purl.org/spar/bido/a-na-wr

:a-na-wr a owl:NamedIndividual , :DiscreteReviewRatingScale ;
	rdfs:comment "Discrete scale from Approved to Not Approved, including Aprproved With Reservations."@en ;
	rdfs:isDefinedBy <http://purl.org/spar/bido-review-measures> ;
	rdfs:label "Approved to Not Approved review rating scale"@en .
# 
# http://purl.org/spar/bido/a-na-wr-app

:a-na-wr-app a owl:NamedIndividual , :ReviewRatingValue ;
	<http://www.w3.org/2004/02/skos/core#closeMatch> :a-r-ts-acc , :dis-0-10-10 , :dis-0-5-4 , :dis-0-5-5 , :dis-n2-p2-pos1 , :dis-n2-p2-pos2 , :sa-sr-bl-acc , :sa-sr-bl-sacc , :sa-sr-nb-acc , :sa-sr-nb-sacc ;
	<http://www.w3.org/2004/02/skos/core#inScheme> :a-na-wr ;
	rdfs:isDefinedBy <http://purl.org/spar/bido-review-measures> ;
	rdfs:label "Approved (Approved to Not Approved review rating scale)"@en .
# 
# http://purl.org/spar/bido/a-na-wr-appwr

:a-na-wr-appwr a owl:NamedIndividual , :ReviewRatingValue ;
	<http://www.w3.org/2004/02/skos/core#closeMatch> :a-r-ts-minrev , :dis-0-5-3 , :sa-sr-bl-wacc , :sa-sr-nb-wacc ;
	<http://www.w3.org/2004/02/skos/core#inScheme> :a-na-wr ;
	rdfs:isDefinedBy <http://purl.org/spar/bido-review-measures> ;
	rdfs:label "Approved with reservations (Approved to Not Approved review rating scale)"@en .
# 
# http://purl.org/spar/bido/a-na-wr-napp

:a-na-wr-napp a owl:NamedIndividual , :ReviewRatingValue ;
	<http://www.w3.org/2004/02/skos/core#closeMatch> :a-r-ts-rej , :dis-0-10-0 , :dis-0-5-0 , :dis-0-5-1 , :dis-n2-p2-neg1 , :dis-n2-p2-neg2 , :sa-sr-bl-rej , :sa-sr-bl-srej , :sa-sr-nb-rej , :sa-sr-nb-srej ;
	<http://www.w3.org/2004/02/skos/core#inScheme> :a-na-wr ;
	rdfs:isDefinedBy <http://purl.org/spar/bido-review-measures> ;
	rdfs:label "Not approved (Approved to Not Approved review rating scale)"@en .
# 
# http://purl.org/spar/bido/a-r-ts

:a-r-ts a owl:NamedIndividual , :DiscreteReviewRatingScale ;
	rdfs:comment "Discrete scale from Accept to Reject, including pre-screening and two strikes rule"@en ;
	rdfs:isDefinedBy <http://purl.org/spar/bido-review-measures> ;
	rdfs:label "Accept to Reject, Two Strikes review rating scale"@en .
# 
# http://purl.org/spar/bido/a-r-ts-acc

:a-r-ts-acc a owl:NamedIndividual , :ReviewRatingValue ;
	<http://www.w3.org/2004/02/skos/core#closeMatch> :a-na-wr-app , :dis-0-10-10 , :dis-0-5-4 , :dis-0-5-5 , :dis-n2-p2-pos1 , :dis-n2-p2-pos2 , :sa-sr-bl-acc , :sa-sr-bl-sacc , :sa-sr-nb-acc , :sa-sr-nb-sacc ;
	<http://www.w3.org/2004/02/skos/core#inScheme> :a-r-ts ;
	rdfs:isDefinedBy <http://purl.org/spar/bido-review-measures> ;
	rdfs:label "Accept (Accept to Reject, Two Strikes review rating scale)"@en .
# 
# http://purl.org/spar/bido/a-r-ts-majrev

:a-r-ts-majrev a owl:NamedIndividual , :ReviewRatingValue ;
	<http://www.w3.org/2004/02/skos/core#closeMatch> :dis-0-10-5 , :dis-n2-p2-0 , :sa-sr-bl-bdl ;
	<http://www.w3.org/2004/02/skos/core#inScheme> :a-r-ts ;
	rdfs:isDefinedBy <http://purl.org/spar/bido-review-measures> ;
	rdfs:label "Major revision (Accept to Reject, Two Strikes review rating scale)"@en .
# 
# http://purl.org/spar/bido/a-r-ts-minrev

:a-r-ts-minrev a owl:NamedIndividual , :ReviewRatingValue ;
	<http://www.w3.org/2004/02/skos/core#closeMatch> :a-na-wr-appwr , :dis-0-5-3 , :sa-sr-bl-wacc , :sa-sr-nb-wacc ;
	<http://www.w3.org/2004/02/skos/core#inScheme> :a-r-ts ;
	rdfs:isDefinedBy <http://purl.org/spar/bido-review-measures> ;
	rdfs:label "Minor revision (Accept to Reject, Two Strikes review rating scale)"@en .
# 
# http://purl.org/spar/bido/a-r-ts-rej

:a-r-ts-rej a owl:NamedIndividual , :ReviewRatingValue ;
	<http://www.w3.org/2004/02/skos/core#closeMatch> :a-na-wr-napp , :dis-0-10-0 , :dis-0-5-0 , :dis-0-5-1 , :dis-n2-p2-neg1 , :dis-n2-p2-neg2 , :sa-sr-bl-rej , :sa-sr-bl-srej , :sa-sr-nb-rej , :sa-sr-nb-srej ;
	<http://www.w3.org/2004/02/skos/core#inScheme> :a-r-ts ;
	rdfs:isDefinedBy <http://purl.org/spar/bido-review-measures> ;
	rdfs:label "Reject (Accept to Reject, Two Strikes review rating scale)"@en .
# 
# http://purl.org/spar/bido/a-r-ts-rejps

:a-r-ts-rejps a owl:NamedIndividual , :ReviewRatingValue ;
	<http://www.w3.org/2004/02/skos/core#inScheme> :a-r-ts ;
	rdfs:isDefinedBy <http://purl.org/spar/bido-review-measures> ;
	rdfs:label "Reject, Pre-Screening (Accept to Reject, Two Strikes review rating scale)"@en .
# 
# http://purl.org/spar/bido/a-r-ts-rejts

:a-r-ts-rejts a owl:NamedIndividual , :ReviewRatingValue ;
	<http://www.w3.org/2004/02/skos/core#inScheme> :a-r-ts ;
	rdfs:isDefinedBy <http://purl.org/spar/bido-review-measures> ;
	rdfs:label "Reject, Two Strikes (Accept to Reject, Two Strikes review rating scale)"@en .
# 
# http://purl.org/spar/bido/acl-1-5

:acl-1-5 a owl:NamedIndividual , :DiscreteReviewerConfidenceScale ;
	rdfs:comment "Discrete scale from 1 to 5, used by Association for Computational Linguistics annual meetings"@en ;
	rdfs:isDefinedBy <http://purl.org/spar/bido-review-measures> ;
	rdfs:label "Discrete 1 to 5 review rating scale"@en .
# 
# http://purl.org/spar/bido/acl-1-5-acl1

:acl-1-5-acl1 a owl:NamedIndividual , :ReviewerConfidenceValue ;
	<http://www.w3.org/2004/02/skos/core#closeMatch> :acl-1-5-acl1 , :ex-null-null ;
	<http://www.w3.org/2004/02/skos/core#inScheme> :acl-1-5 ;
	:hasConfidenceValue "1"^^xsd:int ;
	rdfs:comment "Not reviewer's area of expertise, or paper is very hard to understand. The evaluation is just an educated guess."@en ;
	rdfs:isDefinedBy <http://purl.org/spar/bido-review-measures> ;
	rdfs:label "1 out of 5 (Discrete 1 to 5 review rating scale)"@en .
# 
# http://purl.org/spar/bido/acl-1-5-acl2

:acl-1-5-acl2 a owl:NamedIndividual , :ReviewerConfidenceValue ;
	<http://www.w3.org/2004/02/skos/core#closeMatch> :acl-1-5-acl2 , :ex-null-low ;
	<http://www.w3.org/2004/02/skos/core#inScheme> :acl-1-5 ;
	:hasConfidenceValue "2"^^xsd:int ;
	rdfs:comment "Reviewers is willing to defend my evaluation, but it is fairly likely that he/she missed some details, didn't understand some central points, or can't be sure about the novelty of the work."@en ;
	rdfs:isDefinedBy <http://purl.org/spar/bido-review-measures> ;
	rdfs:label "2 out of 5 (Discrete 1 to 5 review rating scale)"@en .
# 
# http://purl.org/spar/bido/acl-1-5-acl3

:acl-1-5-acl3 a owl:NamedIndividual , :ReviewerConfidenceValue ;
	<http://www.w3.org/2004/02/skos/core#closeMatch> :acl-1-5-acl3 , :ex-null-med ;
	<http://www.w3.org/2004/02/skos/core#inScheme> :acl-1-5 ;
	:hasConfidenceValue "3"^^xsd:int ;
	rdfs:comment "Reviewer is pretty sure, but there's a chance he/she missed something. Although she/he has a good feel for this area in general, she/he did not carefully check the paper's details, e.g., the math, experimental design, or novelty."@en ;
	rdfs:isDefinedBy <http://purl.org/spar/bido-review-measures> ;
	rdfs:label "3 out of 5 (Discrete 1 to 5 review rating scale)"@en .
# 
# http://purl.org/spar/bido/acl-1-5-acl4

:acl-1-5-acl4 a owl:NamedIndividual , :ReviewerConfidenceValue ;
	<http://www.w3.org/2004/02/skos/core#closeMatch> :acl-1-5-acl4 , :ex-null-high ;
	<http://www.w3.org/2004/02/skos/core#inScheme> :acl-1-5 ;
	:hasConfidenceValue "4"^^xsd:int ;
	rdfs:comment "Reviewer is quite sure, tried to check the important points carefully. It's unlikely, though conceivable, that he/she missed something that should affect his/her ratings."@en ;
	rdfs:isDefinedBy <http://purl.org/spar/bido-review-measures> ;
	rdfs:label "4 out of 5 (Discrete 1 to 5 review rating scale)"@en .
# 
# http://purl.org/spar/bido/acl-1-5-acl5

:acl-1-5-acl5 a owl:NamedIndividual , :ReviewerConfidenceValue ;
	<http://www.w3.org/2004/02/skos/core#closeMatch> :acl-1-5-acl5 , :ex-null-exp ;
	<http://www.w3.org/2004/02/skos/core#inScheme> :acl-1-5 ;
	:hasConfidenceValue "5"^^xsd:int ;
	rdfs:comment "Reviewer is positive that the evaluation is correct, has read the paper very carefully and is familiar with related work."@en ;
	rdfs:isDefinedBy <http://purl.org/spar/bido-review-measures> ;
	rdfs:label "5 out of 5 (Discrete 1 to 5 review rating scale)"@en .
# 
# http://purl.org/spar/bido/average-of-reviews-per-paper

:average-of-reviews-per-paper a owl:NamedIndividual , :BibliometricMeasure , _:genid19 .

_:genid19 a owl:Restriction ;
	owl:onProperty _:genid20 .

_:genid20 owl:inverseOf :hasMeasure .

_:genid19 owl:allValuesFrom _:genid21 .

_:genid21 a owl:Restriction ;
	owl:onProperty _:genid22 .

_:genid22 owl:inverseOf :withBibliometricData .

_:genid21 owl:allValuesFrom _:genid23 .

_:genid23 a owl:Restriction ;
	owl:onProperty _:genid24 .

_:genid24 owl:inverseOf :holdsBibliometricDataInTime .

_:genid23 owl:allValuesFrom _:genid25 .

_:genid25 a owl:Class ;
	owl:unionOf _:genid27 .

_:genid27 a rdf:List ;
	rdf:first swc:AcademicEvent ;
	rdf:rest _:genid26 .

_:genid26 a rdf:List ;
	rdf:first fabio:Expression ;
	rdf:rest rdf:nil .

:average-of-reviews-per-paper rdfs:comment "It indicates how many reviewers has been used for each paper submitted to a venue." ;
	rdfs:isDefinedBy <http://purl.org/spar/bido-review-measures> ;
	rdfs:label "average number of reviews per paper" .
# 
# http://purl.org/spar/bido/conference-management-toolkit

:conference-management-toolkit a owl:NamedIndividual , :ScholarlyVenueManagementSystem ;
	rdfs:comment "The Conference Management Toolkit (CMT) is a free conference management service sponsored by Microsoft Research." ;
	rdfs:isDefinedBy <http://purl.org/spar/bido-review-measures> ;
	rdfs:label "Conference Management Toolkit" .
# 
# http://purl.org/spar/bido/core-a

:core-a a owl:NamedIndividual , :ConferenceRankingCategory ;
	:isDefinedIn :core-conference-ranking ;
	:isHigherThan :core-b ;
	rdfs:comment "The CORE category for an excellent conference, and highly respected in a discipline area." ;
	rdfs:isDefinedBy <http://purl.org/spar/bido-review-measures> ;
	rdfs:label "A" .
# 
# http://purl.org/spar/bido/core-a-star

:core-a-star a owl:NamedIndividual , :ConferenceRankingCategory ;
	:isDefinedIn :core-conference-ranking ;
	:isHigherThan :core-a ;
	rdfs:comment "The CORE category for a flagship conference, a leading venue in a discipline area." ;
	rdfs:isDefinedBy <http://purl.org/spar/bido-review-measures> ;
	rdfs:label "A*" .
# 
# http://purl.org/spar/bido/core-b

:core-b a owl:NamedIndividual , :ConferenceRankingCategory ;
	:isDefinedIn :core-conference-ranking ;
	:isHigherThan :core-c ;
	rdfs:comment "The CORE category for a good conference, and well regarded in a discipline area." ;
	rdfs:isDefinedBy <http://purl.org/spar/bido-review-measures> ;
	rdfs:label "B" .
# 
# http://purl.org/spar/bido/core-c

:core-c a owl:NamedIndividual , :ConferenceRankingCategory ;
	:isDefinedIn :core-conference-ranking ;
	:isHigherThan :core-unranked ;
	rdfs:comment "The CORE category for other ranked conference venues that meet minimum standards." ;
	rdfs:isDefinedBy <http://purl.org/spar/bido-review-measures> ;
	rdfs:label "C" .
# 
# http://purl.org/spar/bido/core-conference-ranking

:core-conference-ranking a owl:NamedIndividual , :ConferenceRanking ;
	rdfs:comment "The CORE Conference Ranking (http://www.core.edu.au/index.php/conference-rankings) is an ongoing activity that provides assessments of major conferences in the computing disciplines.The rankings are managed by the CORE Executive Committee, with updates processed from time to time by a subcommittee established as needed." ;
	rdfs:isDefinedBy <http://purl.org/spar/bido-review-measures> ;
	rdfs:label "CORE conference ranking" .
# 
# http://purl.org/spar/bido/core-unranked

:core-unranked a owl:NamedIndividual , :ConferenceRankingCategory ;
	:isDefinedIn :core-conference-ranking ;
	rdfs:comment "The CORE category for a conference for which no ranking decision has been made." ;
	rdfs:isDefinedBy <http://purl.org/spar/bido-review-measures> ;
	rdfs:label "unranked" .
# 
# http://purl.org/spar/bido/demo-paper-accepted

:demo-paper-accepted a owl:NamedIndividual , :BibliometricMeasure , _:genid28 .

_:genid28 a owl:Restriction ;
	owl:onProperty _:genid29 .

_:genid29 owl:inverseOf :hasMeasure .

_:genid28 owl:allValuesFrom _:genid30 .

_:genid30 a owl:Restriction ;
	owl:onProperty _:genid31 .

_:genid31 owl:inverseOf :withBibliometricData .

_:genid30 owl:allValuesFrom _:genid32 .

_:genid32 a owl:Restriction ;
	owl:onProperty _:genid33 .

_:genid33 owl:inverseOf :holdsBibliometricDataInTime .

_:genid32 owl:allValuesFrom _:genid34 .

_:genid34 a owl:Class ;
	owl:unionOf _:genid36 .

_:genid36 a rdf:List ;
	rdf:first swc:AcademicEvent ;
	rdf:rest _:genid35 .

_:genid35 a rdf:List ;
	rdf:first fabio:Expression ;
	rdf:rest rdf:nil .

:demo-paper-accepted rdfs:comment "It indicates how many demo papers has been accepted for publication/presentation in the venue." ;
	rdfs:isDefinedBy <http://purl.org/spar/bido-review-measures> ;
	rdfs:label "number of demo paper accepted" .
# 
# http://purl.org/spar/bido/dis-0-10

:dis-0-10 a owl:NamedIndividual , :DiscreteReviewRatingScale ;
	rdfs:comment "Discrete scale from 0 to 10"@en ;
	rdfs:isDefinedBy <http://purl.org/spar/bido-review-measures> ;
	rdfs:label "Discrete 0 to 10 review rating scale"@en .
# 
# http://purl.org/spar/bido/dis-0-10-0

:dis-0-10-0 a owl:NamedIndividual , :ReviewRatingValue ;
	<http://www.w3.org/2004/02/skos/core#closeMatch> :a-na-wr-napp , :a-r-ts-rej , :dis-0-5-0 , :dis-n2-p2-neg2 , :sa-sr-bl-srej , :sa-sr-nb-srej ;
	<http://www.w3.org/2004/02/skos/core#inScheme> :dis-0-10 ;
	:hasRatingValue "0"^^xsd:int ;
	rdfs:isDefinedBy <http://purl.org/spar/bido-review-measures> ;
	rdfs:label "0 out of 10 (Discrete 0 to 10 review rating scale)"@en .
# 
# http://purl.org/spar/bido/dis-0-10-1

:dis-0-10-1 a owl:NamedIndividual , :ReviewRatingValue ;
	<http://www.w3.org/2004/02/skos/core#inScheme> :dis-0-10 ;
	:hasRatingValue "1"^^xsd:int ;
	rdfs:isDefinedBy <http://purl.org/spar/bido-review-measures> ;
	rdfs:label "1 out of 10 (Discrete 0 to 10 review rating scale)"@en .
# 
# http://purl.org/spar/bido/dis-0-10-10

:dis-0-10-10 a owl:NamedIndividual , :ReviewRatingValue ;
	<http://www.w3.org/2004/02/skos/core#closeMatch> :a-na-wr-app , :a-r-ts-acc , :dis-0-5-5 , :dis-n2-p2-pos2 , :sa-sr-bl-sacc , :sa-sr-nb-sacc ;
	<http://www.w3.org/2004/02/skos/core#inScheme> :dis-0-10 ;
	:hasRatingValue "10"^^xsd:int ;
	rdfs:isDefinedBy <http://purl.org/spar/bido-review-measures> ;
	rdfs:label "10 out of 10 (Discrete 0 to 10 review rating scale)"@en .
# 
# http://purl.org/spar/bido/dis-0-10-2

:dis-0-10-2 a owl:NamedIndividual , :ReviewRatingValue ;
	<http://www.w3.org/2004/02/skos/core#inScheme> :dis-0-10 ;
	:hasRatingValue "2"^^xsd:int ;
	rdfs:isDefinedBy <http://purl.org/spar/bido-review-measures> ;
	rdfs:label "2 out of 10 (Discrete 0 to 10 review rating scale)"@en .
# 
# http://purl.org/spar/bido/dis-0-10-3

:dis-0-10-3 a owl:NamedIndividual , :ReviewRatingValue ;
	<http://www.w3.org/2004/02/skos/core#inScheme> :dis-0-10 ;
	:hasRatingValue "3"^^xsd:int ;
	rdfs:isDefinedBy <http://purl.org/spar/bido-review-measures> ;
	rdfs:label "3 out of 10 (Discrete 0 to 10 review rating scale)"@en .
# 
# http://purl.org/spar/bido/dis-0-10-4

:dis-0-10-4 a owl:NamedIndividual , :ReviewRatingValue ;
	<http://www.w3.org/2004/02/skos/core#inScheme> :dis-0-10 ;
	:hasRatingValue "4"^^xsd:int ;
	rdfs:isDefinedBy <http://purl.org/spar/bido-review-measures> ;
	rdfs:label "4 out of 10 (Discrete 0 to 10 review rating scale)"@en .
# 
# http://purl.org/spar/bido/dis-0-10-5

:dis-0-10-5 a owl:NamedIndividual , :ReviewRatingValue ;
	<http://www.w3.org/2004/02/skos/core#closeMatch> :a-r-ts-majrev , :dis-n2-p2-0 , :sa-sr-bl-bdl ;
	<http://www.w3.org/2004/02/skos/core#inScheme> :dis-0-10 ;
	:hasRatingValue "5"^^xsd:int ;
	rdfs:isDefinedBy <http://purl.org/spar/bido-review-measures> ;
	rdfs:label "5 out of 10 (Discrete 0 to 10 review rating scale)"@en .
# 
# http://purl.org/spar/bido/dis-0-10-6

:dis-0-10-6 a owl:NamedIndividual , :ReviewRatingValue ;
	<http://www.w3.org/2004/02/skos/core#inScheme> :dis-0-10 ;
	:hasRatingValue "6"^^xsd:int ;
	rdfs:isDefinedBy <http://purl.org/spar/bido-review-measures> ;
	rdfs:label "6 out of 10 (Discrete 0 to 10 review rating scale)"@en .
# 
# http://purl.org/spar/bido/dis-0-10-7

:dis-0-10-7 a owl:NamedIndividual , :ReviewRatingValue ;
	<http://www.w3.org/2004/02/skos/core#inScheme> :dis-0-10 ;
	:hasRatingValue "7"^^xsd:int ;
	rdfs:isDefinedBy <http://purl.org/spar/bido-review-measures> ;
	rdfs:label "7 out of 10 (Discrete 0 to 10 review rating scale)"@en .
# 
# http://purl.org/spar/bido/dis-0-10-8

:dis-0-10-8 a owl:NamedIndividual , :ReviewRatingValue ;
	<http://www.w3.org/2004/02/skos/core#inScheme> :dis-0-10 ;
	:hasRatingValue "8"^^xsd:int ;
	rdfs:isDefinedBy <http://purl.org/spar/bido-review-measures> ;
	rdfs:label "8 out of 10 (Discrete 0 to 10 review rating scale)"@en .
# 
# http://purl.org/spar/bido/dis-0-10-9

:dis-0-10-9 a owl:NamedIndividual , :ReviewRatingValue ;
	<http://www.w3.org/2004/02/skos/core#inScheme> :dis-0-10 ;
	:hasRatingValue "9"^^xsd:int ;
	rdfs:isDefinedBy <http://purl.org/spar/bido-review-measures> ;
	rdfs:label "9 out of 10 (Discrete 0 to 10 review rating scale)"@en .
# 
# http://purl.org/spar/bido/dis-0-5

:dis-0-5 a owl:NamedIndividual , :DiscreteReviewRatingScale ;
	rdfs:comment "Discrete scale from 0 to 5"@en ;
	rdfs:isDefinedBy <http://purl.org/spar/bido-review-measures> ;
	rdfs:label "Discrete 0 to 5 review rating scale"@en .
# 
# http://purl.org/spar/bido/dis-0-5-0

:dis-0-5-0 a owl:NamedIndividual , :ReviewRatingValue ;
	<http://www.w3.org/2004/02/skos/core#closeMatch> :a-na-wr-napp , :a-r-ts-rej , :dis-0-10-0 , :dis-n2-p2-neg2 , :sa-sr-bl-srej , :sa-sr-nb-srej ;
	<http://www.w3.org/2004/02/skos/core#inScheme> :dis-0-5 ;
	:hasRatingValue "0"^^xsd:int ;
	rdfs:isDefinedBy <http://purl.org/spar/bido-review-measures> ;
	rdfs:label "0 out of 5 (Discrete 0 to 5 review rating scale)"@en .
# 
# http://purl.org/spar/bido/dis-0-5-1

:dis-0-5-1 a owl:NamedIndividual , :ReviewRatingValue ;
	<http://www.w3.org/2004/02/skos/core#closeMatch> :a-na-wr-napp , :a-r-ts-rej , :dis-n2-p2-neg1 , :sa-sr-bl-rej , :sa-sr-nb-rej ;
	<http://www.w3.org/2004/02/skos/core#inScheme> :dis-0-5 ;
	:hasRatingValue "1"^^xsd:int ;
	rdfs:isDefinedBy <http://purl.org/spar/bido-review-measures> ;
	rdfs:label "1 out of 5 (Discrete 0 to 5 review rating scale)"@en .
# 
# http://purl.org/spar/bido/dis-0-5-2

:dis-0-5-2 a owl:NamedIndividual , :ReviewRatingValue ;
	<http://www.w3.org/2004/02/skos/core#closeMatch> :sa-sr-bl-wrej , :sa-sr-nb-wrej ;
	<http://www.w3.org/2004/02/skos/core#inScheme> :dis-0-5 ;
	:hasRatingValue "2"^^xsd:int ;
	rdfs:isDefinedBy <http://purl.org/spar/bido-review-measures> ;
	rdfs:label "2 out of 5 (Discrete 0 to 5 review rating scale)"@en .
# 
# http://purl.org/spar/bido/dis-0-5-3

:dis-0-5-3 a owl:NamedIndividual , :ReviewRatingValue ;
	<http://www.w3.org/2004/02/skos/core#closeMatch> :a-na-wr-appwr , :a-r-ts-minrev , :sa-sr-bl-wacc , :sa-sr-nb-wacc ;
	<http://www.w3.org/2004/02/skos/core#inScheme> :dis-0-5 ;
	:hasRatingValue "3"^^xsd:int ;
	rdfs:isDefinedBy <http://purl.org/spar/bido-review-measures> ;
	rdfs:label "3 out of 5 (Discrete 0 to 5 review rating scale)"@en .
# 
# http://purl.org/spar/bido/dis-0-5-4

:dis-0-5-4 a owl:NamedIndividual , :ReviewRatingValue ;
	<http://www.w3.org/2004/02/skos/core#closeMatch> :a-na-wr-app , :a-r-ts-acc , :dis-n2-p2-pos1 , :sa-sr-bl-acc , :sa-sr-nb-acc ;
	<http://www.w3.org/2004/02/skos/core#inScheme> :dis-0-5 ;
	:hasRatingValue "4"^^xsd:int ;
	rdfs:isDefinedBy <http://purl.org/spar/bido-review-measures> ;
	rdfs:label "4 out of 5 (Discrete 0 to 5 review rating scale)"@en .
# 
# http://purl.org/spar/bido/dis-0-5-5

:dis-0-5-5 a owl:NamedIndividual , :ReviewRatingValue ;
	<http://www.w3.org/2004/02/skos/core#closeMatch> :a-na-wr-app , :a-r-ts-acc , :dis-0-10-10 , :dis-n2-p2-pos2 , :sa-sr-bl-sacc , :sa-sr-nb-sacc ;
	<http://www.w3.org/2004/02/skos/core#inScheme> :dis-0-5 ;
	:hasRatingValue "5"^^xsd:int ;
	rdfs:isDefinedBy <http://purl.org/spar/bido-review-measures> ;
	rdfs:label "5 out of 5 (Discrete 0 to 5 review rating scale)"@en .
# 
# http://purl.org/spar/bido/dis-n2-p2

:dis-n2-p2 a owl:NamedIndividual , :DiscreteReviewRatingScale ;
	rdfs:comment "Discrete scale from -2 to 2, including 0"@en ;
	rdfs:isDefinedBy <http://purl.org/spar/bido-review-measures> ;
	rdfs:label "Discrete -2 to 2 review rating scale"@en .
# 
# http://purl.org/spar/bido/dis-n2-p2-0

:dis-n2-p2-0 a owl:NamedIndividual , :ReviewRatingValue ;
	<http://www.w3.org/2004/02/skos/core#closeMatch> :a-r-ts-majrev , :dis-0-10-5 , :sa-sr-bl-bdl ;
	<http://www.w3.org/2004/02/skos/core#inScheme> :dis-n2-p2 ;
	:hasRatingValue "0"^^xsd:int ;
	rdfs:isDefinedBy <http://purl.org/spar/bido-review-measures> ;
	rdfs:label "0 on a [-2,2] scale (Discrete -2 to 2 review rating scale)"@en .
# 
# http://purl.org/spar/bido/dis-n2-p2-neg1

:dis-n2-p2-neg1 a owl:NamedIndividual , :ReviewRatingValue ;
	<http://www.w3.org/2004/02/skos/core#closeMatch> :a-na-wr-napp , :a-r-ts-rej , :dis-0-5-1 , :sa-sr-bl-rej , :sa-sr-nb-rej ;
	<http://www.w3.org/2004/02/skos/core#inScheme> :dis-n2-p2 ;
	:hasRatingValue "-1"^^xsd:int ;
	rdfs:isDefinedBy <http://purl.org/spar/bido-review-measures> ;
	rdfs:label "-1 on a [-2,2] scale (Discrete -2 to 2 review rating scale)"@en .
# 
# http://purl.org/spar/bido/dis-n2-p2-neg2

:dis-n2-p2-neg2 a owl:NamedIndividual , :ReviewRatingValue ;
	<http://www.w3.org/2004/02/skos/core#closeMatch> :a-na-wr-napp , :a-r-ts-rej , :dis-0-10-0 , :dis-0-5-0 , :sa-sr-bl-srej , :sa-sr-nb-srej ;
	<http://www.w3.org/2004/02/skos/core#inScheme> :dis-n2-p2 ;
	:hasRatingValue "-2"^^xsd:int ;
	rdfs:isDefinedBy <http://purl.org/spar/bido-review-measures> ;
	rdfs:label "-2 on a [-2,2] scale (Discrete -2 to 2 review rating scale)"@en .
# 
# http://purl.org/spar/bido/dis-n2-p2-pos1

:dis-n2-p2-pos1 a owl:NamedIndividual , :ReviewRatingValue ;
	<http://www.w3.org/2004/02/skos/core#closeMatch> :a-na-wr-app , :a-r-ts-acc , :dis-0-5-4 , :sa-sr-bl-acc , :sa-sr-nb-acc ;
	<http://www.w3.org/2004/02/skos/core#inScheme> :dis-n2-p2 ;
	:hasRatingValue "1"^^xsd:int ;
	rdfs:isDefinedBy <http://purl.org/spar/bido-review-measures> ;
	rdfs:label "1 on a [-2,2] scale (Discrete -2 to 2 review rating scale)"@en .
# 
# http://purl.org/spar/bido/dis-n2-p2-pos2

:dis-n2-p2-pos2 a owl:NamedIndividual , :ReviewRatingValue ;
	<http://www.w3.org/2004/02/skos/core#closeMatch> :a-na-wr-app , :a-r-ts-acc , :dis-0-10-10 , :dis-0-5-5 , :sa-sr-bl-sacc , :sa-sr-nb-sacc ;
	<http://www.w3.org/2004/02/skos/core#inScheme> :dis-n2-p2 ;
	:hasRatingValue "2"^^xsd:int ;
	rdfs:isDefinedBy <http://purl.org/spar/bido-review-measures> ;
	rdfs:label "2 on a [-2,2] scale (Discrete -2 to 2 review rating scale)"@en .
# 
# http://purl.org/spar/bido/double-blind-peer-review

:double-blind-peer-review a owl:NamedIndividual , :PeerReviewType ;
	rdfs:comment "It identifies all the review processes where the identity of the authors is concealed from the reviewers, and vice versa." ;
	rdfs:isDefinedBy <http://purl.org/spar/bido-review-measures> ;
	rdfs:label "double blind peer review" .
# 
# http://purl.org/spar/bido/easychair

:easychair a owl:NamedIndividual , :ScholarlyVenueManagementSystem ;
	rdfs:comment "EasyChair is a conference management system that is flexible, easy to use, and has many features to make it suitable for various conference models. It is currently probably the most commonly used conference management system." ;
	rdfs:isDefinedBy <http://purl.org/spar/bido-review-measures> ;
	rdfs:label "EasyChair" .
# 
# http://purl.org/spar/bido/ex-null

:ex-null a owl:NamedIndividual , :DiscreteReviewerConfidenceScale ;
	rdfs:comment "Discrete scale from Expert to Null, also representend in an scale from 4 to 0"@en ;
	rdfs:isDefinedBy <http://purl.org/spar/bido-review-measures> ;
	rdfs:label "Expert to Null reviewer confidence scale"@en .
# 
# http://purl.org/spar/bido/ex-null-exp

:ex-null-exp a owl:NamedIndividual , :ReviewerConfidenceValue ;
	<http://www.w3.org/2004/02/skos/core#closeMatch> :acl-1-5-acl5 , :ex-null-exp ;
	<http://www.w3.org/2004/02/skos/core#inScheme> :ex-null ;
	:hasConfidenceValue "4"^^xsd:int ;
	rdfs:isDefinedBy <http://purl.org/spar/bido-review-measures> ;
	rdfs:label "Expert (Expert to Null reviewer confidence scale)"@en .
# 
# http://purl.org/spar/bido/ex-null-high

:ex-null-high a owl:NamedIndividual , :ReviewerConfidenceValue ;
	<http://www.w3.org/2004/02/skos/core#closeMatch> :acl-1-5-acl4 , :ex-null-high ;
	<http://www.w3.org/2004/02/skos/core#inScheme> :ex-null ;
	:hasConfidenceValue "3"^^xsd:int ;
	rdfs:isDefinedBy <http://purl.org/spar/bido-review-measures> ;
	rdfs:label "High (Expert to Null reviewer confidence scale)"@en .
# 
# http://purl.org/spar/bido/ex-null-low

:ex-null-low a owl:NamedIndividual , :ReviewerConfidenceValue ;
	<http://www.w3.org/2004/02/skos/core#closeMatch> :acl-1-5-acl2 , :ex-null-low ;
	<http://www.w3.org/2004/02/skos/core#inScheme> :ex-null ;
	:hasConfidenceValue "1"^^xsd:int ;
	rdfs:isDefinedBy <http://purl.org/spar/bido-review-measures> ;
	rdfs:label "Low (Expert to Null reviewer confidence scale)"@en .
# 
# http://purl.org/spar/bido/ex-null-med

:ex-null-med a owl:NamedIndividual , :ReviewerConfidenceValue ;
	<http://www.w3.org/2004/02/skos/core#closeMatch> :acl-1-5-acl3 , :ex-null-med ;
	<http://www.w3.org/2004/02/skos/core#inScheme> :ex-null ;
	:hasConfidenceValue "2"^^xsd:int ;
	rdfs:isDefinedBy <http://purl.org/spar/bido-review-measures> ;
	rdfs:label "Medium (Expert to Null reviewer confidence scale)"@en .
# 
# http://purl.org/spar/bido/ex-null-null

:ex-null-null a owl:NamedIndividual , :ReviewerConfidenceValue ;
	<http://www.w3.org/2004/02/skos/core#closeMatch> :acl-1-5-acl1 , :ex-null-null ;
	<http://www.w3.org/2004/02/skos/core#inScheme> :ex-null ;
	:hasConfidenceValue "0"^^xsd:int ;
	rdfs:isDefinedBy <http://purl.org/spar/bido-review-measures> ;
	rdfs:label "Null (Expert to Null reviewer confidence scale)"@en .
# 
# http://purl.org/spar/bido/external-reviewers-involved

:external-reviewers-involved a owl:NamedIndividual , :BibliometricMeasure , _:genid37 .

_:genid37 a owl:Restriction ;
	owl:onProperty _:genid38 .

_:genid38 owl:inverseOf :hasMeasure .

_:genid37 owl:allValuesFrom _:genid39 .

_:genid39 a owl:Restriction ;
	owl:onProperty _:genid40 .

_:genid40 owl:inverseOf :withBibliometricData .

_:genid39 owl:allValuesFrom _:genid41 .

_:genid41 a owl:Restriction ;
	owl:onProperty _:genid42 .

_:genid42 owl:inverseOf :holdsBibliometricDataInTime .

_:genid41 owl:allValuesFrom _:genid43 .

_:genid43 a owl:Class ;
	owl:unionOf _:genid45 .

_:genid45 a rdf:List ;
	rdf:first swc:AcademicEvent ;
	rdf:rest _:genid44 .

_:genid44 a rdf:List ;
	rdf:first fabio:Expression ;
	rdf:rest rdf:nil .

:external-reviewers-involved rdfs:comment "It indicates how many external reviewers have been involved in the reviewing phase." ;
	rdfs:isDefinedBy <http://purl.org/spar/bido-review-measures> ;
	rdfs:label "number of external reviewers involved" .
# 
# http://purl.org/spar/bido/full-papers-accepted

:full-papers-accepted a owl:NamedIndividual , :BibliometricMeasure , _:genid46 .

_:genid46 a owl:Restriction ;
	owl:onProperty _:genid47 .

_:genid47 owl:inverseOf :hasMeasure .

_:genid46 owl:allValuesFrom _:genid48 .

_:genid48 a owl:Restriction ;
	owl:onProperty _:genid49 .

_:genid49 owl:inverseOf :withBibliometricData .

_:genid48 owl:allValuesFrom _:genid50 .

_:genid50 a owl:Restriction ;
	owl:onProperty _:genid51 .

_:genid51 owl:inverseOf :holdsBibliometricDataInTime .

_:genid50 owl:allValuesFrom _:genid52 .

_:genid52 a owl:Class ;
	owl:unionOf _:genid54 .

_:genid54 a rdf:List ;
	rdf:first swc:AcademicEvent ;
	rdf:rest _:genid53 .

_:genid53 a rdf:List ;
	rdf:first fabio:Expression ;
	rdf:rest rdf:nil .

:full-papers-accepted rdfs:comment "It indicates how many full papers has been accepted for publication/presentation in the venue." ;
	rdfs:isDefinedBy <http://purl.org/spar/bido-review-measures> ;
	rdfs:label "number of full paper accepted" .
# 
# http://purl.org/spar/bido/open-peer-review

:open-peer-review a owl:NamedIndividual , :PeerReviewType ;
	rdfs:comment "It identifies all the review processes where the identity of the authors and the reviewers is known." ;
	rdfs:isDefinedBy <http://purl.org/spar/bido-review-measures> ;
	rdfs:label "open peer review" .
# 
# http://purl.org/spar/bido/poster-papers-accepted

:poster-papers-accepted a owl:NamedIndividual , :BibliometricMeasure , _:genid55 .

_:genid55 a owl:Restriction ;
	owl:onProperty _:genid56 .

_:genid56 owl:inverseOf :hasMeasure .

_:genid55 owl:allValuesFrom _:genid57 .

_:genid57 a owl:Restriction ;
	owl:onProperty _:genid58 .

_:genid58 owl:inverseOf :withBibliometricData .

_:genid57 owl:allValuesFrom _:genid59 .

_:genid59 a owl:Restriction ;
	owl:onProperty _:genid60 .

_:genid60 owl:inverseOf :holdsBibliometricDataInTime .

_:genid59 owl:allValuesFrom _:genid61 .

_:genid61 a owl:Class ;
	owl:unionOf _:genid63 .

_:genid63 a rdf:List ;
	rdf:first swc:AcademicEvent ;
	rdf:rest _:genid62 .

_:genid62 a rdf:List ;
	rdf:first fabio:Expression ;
	rdf:rest rdf:nil .

:poster-papers-accepted rdfs:comment "It indicates how many poster papers has been accepted for publication/presentation in the venue." ;
	rdfs:isDefinedBy <http://purl.org/spar/bido-review-measures> ;
	rdfs:label "number of poster paper accepted" .
# 
# http://purl.org/spar/bido/sa-sr-bl

:sa-sr-bl a owl:NamedIndividual , :DiscreteReviewRatingScale ;
	rdfs:comment "Discrete scale from Strong Reject to Strong Accept, including Bordeline"@en ;
	rdfs:isDefinedBy <http://purl.org/spar/bido-review-measures> ;
	rdfs:label "Strong Reject to Strong Accept review rating scale"@en .
# 
# http://purl.org/spar/bido/sa-sr-bl-acc

:sa-sr-bl-acc a owl:NamedIndividual , :ReviewRatingValue ;
	<http://www.w3.org/2004/02/skos/core#closeMatch> :a-na-wr-app , :a-r-ts-acc , :dis-0-5-4 , :dis-n2-p2-pos1 , :sa-sr-nb-acc ;
	<http://www.w3.org/2004/02/skos/core#inScheme> :sa-sr-bl ;
	rdfs:isDefinedBy <http://purl.org/spar/bido-review-measures> ;
	rdfs:label "Accept (Strong Reject to Strong Accept review rating scale)"@en .
# 
# http://purl.org/spar/bido/sa-sr-bl-bdl

:sa-sr-bl-bdl a owl:NamedIndividual , :ReviewRatingValue ;
	<http://www.w3.org/2004/02/skos/core#closeMatch> :a-r-ts-majrev , :dis-0-10-5 , :dis-n2-p2-0 ;
	<http://www.w3.org/2004/02/skos/core#inScheme> :sa-sr-bl ;
	rdfs:isDefinedBy <http://purl.org/spar/bido-review-measures> ;
	rdfs:label "Borderline (Strong Reject to Strong Accept review rating scale)"@en .
# 
# http://purl.org/spar/bido/sa-sr-bl-rej

:sa-sr-bl-rej a owl:NamedIndividual , :ReviewRatingValue ;
	<http://www.w3.org/2004/02/skos/core#closeMatch> :a-na-wr-napp , :a-r-ts-rej , :dis-0-5-1 , :dis-n2-p2-neg1 , :sa-sr-nb-rej ;
	<http://www.w3.org/2004/02/skos/core#inScheme> :sa-sr-bl ;
	rdfs:isDefinedBy <http://purl.org/spar/bido-review-measures> ;
	rdfs:label "Reject (Strong Reject to Strong Accept review rating scale)"@en .
# 
# http://purl.org/spar/bido/sa-sr-bl-sacc

:sa-sr-bl-sacc a owl:NamedIndividual , :ReviewRatingValue ;
	<http://www.w3.org/2004/02/skos/core#closeMatch> :a-na-wr-app , :a-r-ts-acc , :dis-0-10-10 , :dis-0-5-5 , :dis-n2-p2-pos2 , :sa-sr-nb-sacc ;
	<http://www.w3.org/2004/02/skos/core#inScheme> :sa-sr-bl ;
	rdfs:isDefinedBy <http://purl.org/spar/bido-review-measures> ;
	rdfs:label "Strong Accept (Strong Reject to Strong Accept review rating scale)"@en .
# 
# http://purl.org/spar/bido/sa-sr-bl-srej

:sa-sr-bl-srej a owl:NamedIndividual , :ReviewRatingValue ;
	<http://www.w3.org/2004/02/skos/core#closeMatch> :a-na-wr-napp , :a-r-ts-rej , :dis-0-10-0 , :dis-0-5-0 , :dis-n2-p2-neg2 , :sa-sr-nb-srej ;
	<http://www.w3.org/2004/02/skos/core#inScheme> :sa-sr-bl ;
	rdfs:isDefinedBy <http://purl.org/spar/bido-review-measures> ;
	rdfs:label "Strong Reject (Strong Reject to Strong Accept review rating scale)"@en .
# 
# http://purl.org/spar/bido/sa-sr-bl-wacc

:sa-sr-bl-wacc a owl:NamedIndividual , :ReviewRatingValue ;
	<http://www.w3.org/2004/02/skos/core#closeMatch> :a-na-wr-appwr , :a-r-ts-minrev , :dis-0-5-3 , :sa-sr-nb-wacc ;
	<http://www.w3.org/2004/02/skos/core#inScheme> :sa-sr-bl ;
	rdfs:isDefinedBy <http://purl.org/spar/bido-review-measures> ;
	rdfs:label "Weak Accept (Strong Reject to Strong Accept review rating scale)"@en .
# 
# http://purl.org/spar/bido/sa-sr-bl-wrej

:sa-sr-bl-wrej a owl:NamedIndividual , :ReviewRatingValue ;
	<http://www.w3.org/2004/02/skos/core#closeMatch> :dis-0-5-2 , :sa-sr-nb-wrej ;
	<http://www.w3.org/2004/02/skos/core#inScheme> :sa-sr-bl ;
	rdfs:isDefinedBy <http://purl.org/spar/bido-review-measures> ;
	rdfs:label "Weak Reject (Strong Reject to Strong Accept review rating scale)"@en .
# 
# http://purl.org/spar/bido/sa-sr-nb

:sa-sr-nb a owl:NamedIndividual , :DiscreteReviewRatingScale ;
	rdfs:comment "Discrete scale from Strong Reject to Strong Accept, excluding Bordeline"@en ;
	rdfs:isDefinedBy <http://purl.org/spar/bido-review-measures> ;
	rdfs:label "Strong Reject to Strong Accept, without Borderline review rating scale"@en .
# 
# http://purl.org/spar/bido/sa-sr-nb-acc

:sa-sr-nb-acc a owl:NamedIndividual , :ReviewRatingValue ;
	<http://www.w3.org/2004/02/skos/core#closeMatch> :a-na-wr-app , :a-r-ts-acc , :dis-0-10-10 , :dis-0-5-4 , :dis-n2-p2-pos1 , :sa-sr-bl-acc ;
	<http://www.w3.org/2004/02/skos/core#inScheme> :sa-sr-nb ;
	rdfs:isDefinedBy <http://purl.org/spar/bido-review-measures> ;
	rdfs:label "Accept (Strong Reject to Strong Accept, without Borderline review rating scale)"@en .
# 
# http://purl.org/spar/bido/sa-sr-nb-rej

:sa-sr-nb-rej a owl:NamedIndividual , :ReviewRatingValue ;
	<http://www.w3.org/2004/02/skos/core#closeMatch> :a-na-wr-napp , :a-r-ts-rej , :dis-0-10-0 , :dis-0-5-1 , :dis-n2-p2-neg1 , :sa-sr-bl-rej ;
	<http://www.w3.org/2004/02/skos/core#inScheme> :sa-sr-nb ;
	rdfs:isDefinedBy <http://purl.org/spar/bido-review-measures> ;
	rdfs:label "Reject (Strong Reject to Strong Accept, without Borderline review rating scale)"@en .
# 
# http://purl.org/spar/bido/sa-sr-nb-sacc

:sa-sr-nb-sacc a owl:NamedIndividual , :ReviewRatingValue ;
	<http://www.w3.org/2004/02/skos/core#closeMatch> :a-na-wr-app , :a-r-ts-acc , :dis-0-10-10 , :dis-0-5-5 , :dis-n2-p2-pos2 , :sa-sr-bl-sacc ;
	<http://www.w3.org/2004/02/skos/core#inScheme> :sa-sr-nb ;
	rdfs:isDefinedBy <http://purl.org/spar/bido-review-measures> ;
	rdfs:label "Strong Accept (Strong Reject to Strong Accept, without Borderline review rating scale)"@en .
# 
# http://purl.org/spar/bido/sa-sr-nb-srej

:sa-sr-nb-srej a owl:NamedIndividual , :ReviewRatingValue ;
	<http://www.w3.org/2004/02/skos/core#closeMatch> :a-na-wr-napp , :a-r-ts-rej , :dis-0-10-0 , :dis-0-5-0 , :dis-n2-p2-neg2 , :sa-sr-bl-srej ;
	<http://www.w3.org/2004/02/skos/core#inScheme> :sa-sr-nb ;
	rdfs:isDefinedBy <http://purl.org/spar/bido-review-measures> ;
	rdfs:label "Strong Reject (Strong Reject to Strong Accept, without Borderline review rating scale)"@en .
# 
# http://purl.org/spar/bido/sa-sr-nb-wacc

:sa-sr-nb-wacc a owl:NamedIndividual , :ReviewRatingValue ;
	<http://www.w3.org/2004/02/skos/core#closeMatch> :a-na-wr-appwr , :a-r-ts-minrev , :dis-0-5-3 , :sa-sr-bl-wacc ;
	<http://www.w3.org/2004/02/skos/core#inScheme> :sa-sr-nb ;
	rdfs:isDefinedBy <http://purl.org/spar/bido-review-measures> ;
	rdfs:label "Weak Accept (Strong Reject to Strong Accept, without Borderline review rating scale)"@en .
# 
# http://purl.org/spar/bido/sa-sr-nb-wrej

:sa-sr-nb-wrej a owl:NamedIndividual , :ReviewRatingValue ;
	<http://www.w3.org/2004/02/skos/core#closeMatch> :dis-0-5-2 , :sa-sr-bl-wrej ;
	<http://www.w3.org/2004/02/skos/core#inScheme> :sa-sr-nb ;
	rdfs:isDefinedBy <http://purl.org/spar/bido-review-measures> ;
	rdfs:label "Weak Reject (Strong Reject to Strong Accept, without Borderline review rating scale)"@en .
# 
# http://purl.org/spar/bido/short-papers-accepted

:short-papers-accepted a owl:NamedIndividual , :BibliometricMeasure , _:genid64 .

_:genid64 a owl:Restriction ;
	owl:onProperty _:genid65 .

_:genid65 owl:inverseOf :hasMeasure .

_:genid64 owl:allValuesFrom _:genid66 .

_:genid66 a owl:Restriction ;
	owl:onProperty _:genid67 .

_:genid67 owl:inverseOf :withBibliometricData .

_:genid66 owl:allValuesFrom _:genid68 .

_:genid68 a owl:Restriction ;
	owl:onProperty _:genid69 .

_:genid69 owl:inverseOf :holdsBibliometricDataInTime .

_:genid68 owl:allValuesFrom _:genid70 .

_:genid70 a owl:Class ;
	owl:unionOf _:genid72 .

_:genid72 a rdf:List ;
	rdf:first swc:AcademicEvent ;
	rdf:rest _:genid71 .

_:genid71 a rdf:List ;
	rdf:first fabio:Expression ;
	rdf:rest rdf:nil .

:short-papers-accepted rdfs:comment "It indicates how many short papers has been accepted for publication/presentation in the venue." ;
	rdfs:isDefinedBy <http://purl.org/spar/bido-review-measures> ;
	rdfs:label "number of short paper accepted" .
# 
# http://purl.org/spar/bido/single-blind-peer-review

:single-blind-peer-review a owl:NamedIndividual , :PeerReviewType ;
	rdfs:comment "It identifies all the review processes where the identity of the reviewers is concealed from the authors." ;
	rdfs:isDefinedBy <http://purl.org/spar/bido-review-measures> ;
	rdfs:label "single blind peer review" .
# 
# http://purl.org/spar/bido/submissions-sent-for-review

:submissions-sent-for-review a owl:NamedIndividual , :BibliometricMeasure , _:genid73 .

_:genid73 a owl:Restriction ;
	owl:onProperty _:genid74 .

_:genid74 owl:inverseOf :hasMeasure .

_:genid73 owl:allValuesFrom _:genid75 .

_:genid75 a owl:Restriction ;
	owl:onProperty _:genid76 .

_:genid76 owl:inverseOf :withBibliometricData .

_:genid75 owl:allValuesFrom _:genid77 .

_:genid77 a owl:Restriction ;
	owl:onProperty _:genid78 .

_:genid78 owl:inverseOf :holdsBibliometricDataInTime .

_:genid77 owl:allValuesFrom _:genid79 .

_:genid79 a owl:Class ;
	owl:unionOf _:genid81 .

_:genid81 a rdf:List ;
	rdf:first swc:AcademicEvent ;
	rdf:rest _:genid80 .

_:genid80 a rdf:List ;
	rdf:first fabio:Expression ;
	rdf:rest rdf:nil .

:submissions-sent-for-review rdfs:comment "It indicates how many submitted papers has been assagned to reviewers for revision." ;
	rdfs:isDefinedBy <http://purl.org/spar/bido-review-measures> ;
	rdfs:label "number of submission sent for review" .
# 
# http://purl.org/spar/bido/to-10-continuos

:to-10-continuos a owl:NamedIndividual , :ReviewRatingScale ;
	rdfs:isDefinedBy <http://purl.org/spar/bido-review-measures> ;
	rdfs:label "0 to 10 continuos review rating scale"@en .
# 
# http://purl.org/spar/bido/to-15-continuos

:to-15-continuos a owl:NamedIndividual , :ReviewRatingScale ;
	rdfs:isDefinedBy <http://purl.org/spar/bido-review-measures> ;
	rdfs:label "0 to 15 continuos review rating scale"@en .
# 
# http://purl.org/spar/bido/to-5-continuos

:to-5-continuos a owl:NamedIndividual , :ReviewRatingScale ;
	rdfs:isDefinedBy <http://purl.org/spar/bido-review-measures> ;
	<http://www.w3.org/2004/02/skos/core#prefLabel> "0 to 5 continuos review rating scale"@en .
# 
# Generated by the OWL API (version 4.2.6.20160910-2108) https://github.com/owlcs/owlapi
